nleft -> depth

PEG.v
@@ -760,92 +760,92 @@ Inductive verifyrule :
   grammar -> pat -> nat -> bool -> option bool -> list nat -> Prop :=
 
   | VREmpty :
-      forall g nleft nb,
-      verifyrule g PEmpty nleft nb (Some true) nil
+      forall g d nb,
+      verifyrule g PEmpty d nb (Some true) nil
   | VRChar :
-      forall g a nleft nb,
-      verifyrule g (PChar a) nleft nb (Some nb) nil
+      forall g a d nb,
+      verifyrule g (PChar a) d nb (Some nb) nil
   | VRAnyChar :
-      forall g nleft nb,
-      verifyrule g PAnyChar nleft nb (Some nb) nil
+      forall g d nb,
+      verifyrule g PAnyChar d nb (Some nb) nil
   | VRSequenceNone :
-      forall g p1 p2 nleft nb v,
-      verifyrule g p1 nleft false None v ->
-      verifyrule g (PSequence p1 p2) nleft nb None v
+      forall g p1 p2 d nb v,
+      verifyrule g p1 d false None v ->
+      verifyrule g (PSequence p1 p2) d nb None v
   | VRSequenceSomeTrue :
-      forall g p1 p2 nleft nb res v1 v2,
-      verifyrule g p1 nleft false (Some true) v1 ->
-      verifyrule g p2 nleft nb res v2 ->
-      verifyrule g (PSequence p1 p2) nleft nb res v2
+      forall g p1 p2 d nb res v1 v2,
+      verifyrule g p1 d false (Some true) v1 ->
+      verifyrule g p2 d nb res v2 ->
+      verifyrule g (PSequence p1 p2) d nb res v2
   | VRSequenceSomeFalse :
-      forall g p1 p2 nleft nb v,
-      verifyrule g p1 nleft false (Some false) v ->
-      verifyrule g (PSequence p1 p2) nleft nb (Some nb) v
+      forall g p1 p2 d nb v,
+      verifyrule g p1 d false (Some false) v ->
+      verifyrule g (PSequence p1 p2) d nb (Some nb) v
   | VRChoiceNone :
-      forall g p1 p2 nleft nb v,
-      verifyrule g p1 nleft nb None v ->
-      verifyrule g (PChoice p1 p2) nleft nb None v
+      forall g p1 p2 d nb v,
+      verifyrule g p1 d nb None v ->
+      verifyrule g (PChoice p1 p2) d nb None v
   | VRChoiceSome :
-      forall g p1 p2 nleft nb nb' res v1 v2,
-      verifyrule g p1 nleft nb (Some nb') v1 ->
-      verifyrule g p2 nleft nb' res v2 ->
-      verifyrule g (PChoice p1 p2) nleft nb res v2
+      forall g p1 p2 d nb nb' res v1 v2,
+      verifyrule g p1 d nb (Some nb') v1 ->
+      verifyrule g p2 d nb' res v2 ->
+      verifyrule g (PChoice p1 p2) d nb res v2
   | VRRepetition :
-      forall g p nleft nb res v,
-      verifyrule g p nleft true res v ->
-      verifyrule g (PRepetition p) nleft nb res v
+      forall g p d nb res v,
+      verifyrule g p d true res v ->
+      verifyrule g (PRepetition p) d nb res v
   | VRNot :
-      forall g p nleft nb res v,
-      verifyrule g p nleft true res v ->
-      verifyrule g (PNot p) nleft nb res v
+      forall g p d nb res v,
+      verifyrule g p d true res v ->
+      verifyrule g (PNot p) d nb res v
   | VRNTZero :
       forall g i nb,
       verifyrule g (PNT i) O nb None nil
   | VRNTSucc :
-      forall g i p nleft nb res v,
+      forall g i p d nb res v,
       nth_error g i = Some p ->
-      verifyrule g p nleft nb res v ->
-      verifyrule g (PNT i) (S nleft) nb res (i :: v)
+      verifyrule g p d nb res v ->
+      verifyrule g (PNT i) (S d) nb res (i :: v)
   .
 
 Goal
-  forall g nb nleft,
-  verifyrule g PEmpty nleft nb (Some true) nil.
+  forall g nb d,
+  verifyrule g PEmpty d nb (Some true) nil.
 Proof.
   eauto using verifyrule.
 Qed.
 
 Goal
-  forall g a nb nleft,
-  verifyrule g (PChar a) nleft nb (Some nb) nil.
+  forall g a nb d,
+  verifyrule g (PChar a) d nb (Some nb) nil.
 Proof.
   eauto using verifyrule.
 Qed.
 
 Goal
-  forall g nb nleft,
-  verifyrule g PAnyChar nleft nb (Some nb) nil.
+  forall g nb d,
+  verifyrule g PAnyChar d nb (Some nb) nil.
 Proof.
   eauto using verifyrule.
 Qed.
 
 Goal
-  forall g nb nleft,
-  verifyrule g (PSequence PEmpty PEmpty) nleft nb (Some true) nil.
+  forall g nb d,
+  verifyrule g (PSequence PEmpty PEmpty) d nb (Some true) nil.
 Proof.
   eauto using verifyrule.
 Qed.
 
 Goal
-  forall g nb nleft,
-  verifyrule g (PSequence PAnyChar PEmpty) nleft nb (Some nb) nil.
+  forall g nb d,
+  verifyrule g (PSequence PAnyChar PEmpty) d nb (Some nb) nil.
 Proof.
   eauto using verifyrule.
 Qed.
 
 Goal
-  forall g nb nleft,
-  verifyrule g (PSequence PEmpty PAnyChar) nleft nb (Some nb) nil.
+  forall g nb d,
+  verifyrule g (PSequence PEmpty PAnyChar) d nb (Some nb) nil.
 Proof.
   eauto using verifyrule.
 Qed.
@@ -887,29 +887,29 @@ Proof.
 Qed.
 
 Goal
-  forall g nb nleft,
-  verifyrule g (PChoice PEmpty PEmpty) nleft nb (Some true) nil.
+  forall g nb d,
+  verifyrule g (PChoice PEmpty PEmpty) d nb (Some true) nil.
 Proof.
   eauto using verifyrule.
 Qed.
 
 Goal
-  forall g nb nleft,
-  verifyrule g (PChoice PAnyChar PEmpty) nleft nb (Some true) nil.
+  forall g nb d,
+  verifyrule g (PChoice PAnyChar PEmpty) d nb (Some true) nil.
 Proof.
   eauto using verifyrule.
 Qed.
 
 Goal
-  forall g nb nleft,
-  verifyrule g (PChoice PEmpty PAnyChar) nleft nb (Some true) nil.
+  forall g nb d,
+  verifyrule g (PChoice PEmpty PAnyChar) d nb (Some true) nil.
 Proof.
   eauto using verifyrule.
 Qed.
 
 Goal
-  forall g nb nleft,
-  verifyrule g (PChoice PAnyChar PAnyChar) nleft nb (Some nb) nil.
+  forall g nb d,
+  verifyrule g (PChoice PAnyChar PAnyChar) d nb (Some nb) nil.
 Proof.
   eauto using verifyrule.
 Qed.
@@ -1022,22 +1022,22 @@ Proof.
 Qed.
 
 Goal
-  forall nleft,
-  verifyrule [PNT 0] (PNT 0) nleft false None (repeat 0 nleft).
+  forall d,
+  verifyrule [PNT 0] (PNT 0) d false None (repeat 0 d).
 Proof.
   intros.
-  induction nleft.
+  induction d.
   - (* O *)
     eauto using verifyrule.
-  - (* S nleft *)
+  - (* S d *)
     simpl.
     eapply VRNTSucc; simpl; auto.
 Qed.
 
 Lemma verifyrule_determinism :
-  forall g p nleft nb res1 res2 v1 v2,
-  verifyrule g p nleft nb res1 v1 ->
-  verifyrule g p nleft nb res2 v2 ->
+  forall g p d nb res1 res2 v1 v2,
+  verifyrule g p d nb res1 v1 ->
+  verifyrule g p d nb res2 v2 ->
   res1 = res2 /\ v1 = v2.
 Proof.
   intros * H1 H2.
@@ -1049,8 +1049,8 @@ Proof.
   try lia;
   auto;
   try match goal with
-  [ IHx: forall res v, verifyrule ?g ?p ?nleft ?nb res v -> _ = res /\ _ = v,
-    Hx: verifyrule ?g ?p ?nleft ?nb _ _ |- _ ] =>
+  [ IHx: forall res v, verifyrule ?g ?p ?d ?nb res v -> _ = res /\ _ = v,
+    Hx: verifyrule ?g ?p ?d ?nb _ _ |- _ ] =>
       apply IHx in Hx;
       destruct Hx;
       try discriminate;
@@ -1062,18 +1062,18 @@ Qed.
 
 Ltac pose_verifyrule_determinism :=
   repeat match goal with
-    [ Hx1: verifyrule ?g ?p ?nleft ?nb ?res1 ?v1,
-      Hx2: verifyrule ?g ?p ?nleft ?nb ?res2 ?v2 |- _ ] =>
+    [ Hx1: verifyrule ?g ?p ?d ?nb ?res1 ?v1,
+      Hx2: verifyrule ?g ?p ?d ?nb ?res2 ?v2 |- _ ] =>
           assert (res1 = res2 /\ v1 = v2)
           as [? ?]
           by eauto using verifyrule_determinism;
           clear Hx2
   end.
 
-Lemma verifyrule_S_nleft :
-  forall g p nleft nb nb' v,
-  verifyrule g p nleft nb (Some nb') v ->
-  verifyrule g p (S nleft) nb (Some nb') v.
+Lemma verifyrule_S_depth :
+  forall g p d nb nb' v,
+  verifyrule g p d nb (Some nb') v ->
+  verifyrule g p (S d) nb (Some nb') v.
 Proof.
   intros * H.
   remember (Some nb').
@@ -1083,32 +1083,32 @@ Proof.
   eauto using verifyrule.
 Qed.
 
-Lemma verifyrule_nleft_le_some_determinism :
-  forall g p nleft nleft' nb nb' v,
-  verifyrule g p nleft nb (Some nb') v ->
-  nleft <= nleft' ->
-  verifyrule g p nleft' nb (Some nb') v.
+Lemma verifyrule_depth_le_some_determinism :
+  forall g p d d' nb nb' v,
+  verifyrule g p d nb (Some nb') v ->
+  d <= d' ->
+  verifyrule g p d' nb (Some nb') v.
 Proof.
   intros * H Hle.
   induction Hle;
-  eauto using verifyrule_S_nleft.
+  eauto using verifyrule_S_depth.
 Qed.
 
-Lemma verifyrule_nleft_some_determinism :
-  forall g p nleft nleft' nb b b' v v',
-  verifyrule g p nleft nb (Some b) v ->
-  verifyrule g p nleft' nb (Some b') v' ->
+Lemma verifyrule_depth_some_determinism :
+  forall g p d d' nb b b' v v',
+  verifyrule g p d nb (Some b) v ->
+  verifyrule g p d' nb (Some b') v' ->
   b = b' /\ v = v'.
 Proof.
   intros * H H'.
-  destruct (Compare_dec.le_ge_dec nleft nleft') as [Hle|Hge];
+  destruct (Compare_dec.le_ge_dec d d') as [Hle|Hge];
   try unfold ge in *;
   match goal with
-    [ Hx: ?nleft <= ?nleft',
-      Hy: verifyrule ?g ?p ?nleft ?nb (Some ?b) ?v,
-      Hz: verifyrule ?g ?p ?nleft' ?nb (Some ?b') ?v' |- _ ] =>
-          assert (verifyrule g p nleft' nb (Some b) v)
-          by eauto using verifyrule_nleft_le_some_determinism
+    [ Hx: ?d <= ?d',
+      Hy: verifyrule ?g ?p ?d ?nb (Some ?b) ?v,
+      Hz: verifyrule ?g ?p ?d' ?nb (Some ?b') ?v' |- _ ] =>
+          assert (verifyrule g p d' nb (Some b) v)
+          by eauto using verifyrule_depth_le_some_determinism
   end;
   pose_verifyrule_determinism;
   subst;
@@ -1118,27 +1118,27 @@ Qed.
 
 Ltac pose_verifyrule_some_determinism :=
   repeat match goal with
-    [ Hx1: verifyrule ?g ?p ?nleft1 ?nb (Some ?b1) ?v1,
-      Hx2: verifyrule ?g ?p ?nleft2 ?nb (Some ?b2) ?v2 |- _ ] =>
+    [ Hx1: verifyrule ?g ?p ?d1 ?nb (Some ?b1) ?v1,
+      Hx2: verifyrule ?g ?p ?d2 ?nb (Some ?b2) ?v2 |- _ ] =>
           assert (b1 = b2 /\ v1 = v2)
           as [? ?]
-          by eauto using verifyrule_nleft_some_determinism;
+          by eauto using verifyrule_depth_some_determinism;
           clear Hx2
   end.
 
-Lemma verifyrule_length_v_le_nleft :
-  forall g p nleft nb res v,
-  verifyrule g p nleft nb res v ->
-  length v <= nleft.
+Lemma verifyrule_length_v_le_depth :
+  forall g p d nb res v,
+  verifyrule g p d nb res v ->
+  length v <= d.
 Proof.
   intros * H.
   induction H; simpl; lia.
 Qed.
 
-Lemma verifyrule_length_v_eq_nleft :
-  forall g p nleft nb v,
-  verifyrule g p nleft nb None v ->
-  length v = nleft.
+Lemma verifyrule_length_v_eq_depth :
+  forall g p d nb v,
+  verifyrule g p d nb None v ->
+  length v = d.
 Proof.
   intros * H.
   remember None.
@@ -1149,8 +1149,8 @@ Proof.
 Qed.
 
 Lemma verifyrule_i_in_v_lt_length_g :
-  forall g p nleft nb res v i,
-  verifyrule g p nleft nb res v ->
+  forall g p d nb res v i,
+  verifyrule g p d nb res v ->
   In i v ->
   i < length g.
 Proof.
@@ -1170,64 +1170,64 @@ Proof.
   end.
 Qed.
 
-Inductive coherent_return_type_after_nleft_increase : option bool -> option bool -> Prop :=
+Inductive coherent_return_type_after_depth_increase : option bool -> option bool -> Prop :=
   | FromNone :
       forall res,
-      coherent_return_type_after_nleft_increase None res
+      coherent_return_type_after_depth_increase None res
   | FromSome :
       forall b,
-      coherent_return_type_after_nleft_increase (Some b) (Some b)
+      coherent_return_type_after_depth_increase (Some b) (Some b)
   .
 
-Lemma coherent_return_type_after_nleft_increase_transitive :
+Lemma coherent_return_type_after_depth_increase_transitive :
   forall res1 res2 res3,
-  coherent_return_type_after_nleft_increase res1 res2 ->
-  coherent_return_type_after_nleft_increase res2 res3 ->
-  coherent_return_type_after_nleft_increase res1 res3.
+  coherent_return_type_after_depth_increase res1 res2 ->
+  coherent_return_type_after_depth_increase res2 res3 ->
+  coherent_return_type_after_depth_increase res1 res3.
 Proof.
   intros * H12 H23.
   inversion H12; subst;
-  eauto using coherent_return_type_after_nleft_increase.
+  eauto using coherent_return_type_after_depth_increase.
 Qed.
 
-Lemma verifyrule_nleft_decrease :
-  forall g p nleft nb res v,
-  verifyrule g p (S nleft) nb res v ->
+Lemma verifyrule_depth_decrease :
+  forall g p d nb res v,
+  verifyrule g p (S d) nb res v ->
   exists res' v',
-  coherent_return_type_after_nleft_increase res' res /\
-  verifyrule g p nleft nb res' v'.
+  coherent_return_type_after_depth_increase res' res /\
+  verifyrule g p d nb res' v'.
 Proof.
   intros * H.
-  remember (S nleft) as nleft'.
-  generalize dependent nleft.
+  remember (S d) as d'.
+  generalize dependent d.
   induction H;
   intros;
   subst;
   try discriminate;
   try destruct1;
   try match goal with
-    [ IHx: forall nleftx, ?nleft' = S nleftx -> _
-      |- exists _ _, _ /\ verifyrule _ _ ?nleft' _ _ _ ] =>
-          destruct nleft'
+    [ IHx: forall dx, ?d' = S dx -> _
+      |- exists _ _, _ /\ verifyrule _ _ ?d' _ _ _ ] =>
+          destruct d'
   end;
   repeat specialize_forall_eq;
   repeat specialize_eq_refl;
   repeat destruct_exists_hyp;
   repeat destruct_and_hyp;
   try match goal with
-    [ Hx: coherent_return_type_after_nleft_increase _ _ |- _ ] =>
+    [ Hx: coherent_return_type_after_depth_increase _ _ |- _ ] =>
         inversion Hx; subst
   end;
-  eauto using verifyrule, coherent_return_type_after_nleft_increase.
+  eauto using verifyrule, coherent_return_type_after_depth_increase.
 Qed.
 
-Lemma verifyrule_nleft_le_coherent_result_type :
-  forall g p nleft nleft' nb res v,
-  verifyrule g p nleft' nb res v ->
-  nleft <= nleft' ->
+Lemma verifyrule_depth_le_coherent_result_type :
+  forall g p d d' nb res v,
+  verifyrule g p d' nb res v ->
+  d <= d' ->
   exists res' v',
-  coherent_return_type_after_nleft_increase res' res /\
-  verifyrule g p nleft nb res' v'.
+  coherent_return_type_after_depth_increase res' res /\
+  verifyrule g p d nb res' v'.
 Proof.
   intros * Hv Hle.
   generalize dependent v.
@@ -1235,28 +1235,28 @@ Proof.
   generalize dependent nb.
   generalize dependent p.
   generalize dependent g.
-  induction Hle as [|nleft' Hle IH];
+  induction Hle as [|d' Hle IH];
   intros.
-  - (* nleft = nleft', prove for nleft' *)
+  - (* d = d', prove for d' *)
     destruct res;
-    eauto using coherent_return_type_after_nleft_increase.
-  - (* nleft <= nleft', prove for (S nleft') *)
+    eauto using coherent_return_type_after_depth_increase.
+  - (* d <= d', prove for (S d') *)
     assert (exists res' v',
-            coherent_return_type_after_nleft_increase res' res /\
-            verifyrule g p nleft' nb res' v')
+            coherent_return_type_after_depth_increase res' res /\
+            verifyrule g p d' nb res' v')
     as [res' [v' [? ?]]]
-    by eauto using verifyrule_nleft_decrease.
+    by eauto using verifyrule_depth_decrease.
     assert (exists res'' v'',
-            coherent_return_type_after_nleft_increase res'' res' /\
-            verifyrule g p nleft nb res'' v'')
+            coherent_return_type_after_depth_increase res'' res' /\
+            verifyrule g p d nb res'' v'')
     as [res'' [v'' [? ?]]]
     by eauto.
-    eauto using coherent_return_type_after_nleft_increase_transitive.
+    eauto using coherent_return_type_after_depth_increase_transitive.
 Qed.
 
 Lemma verifyrule_res_none_or_some_true :
-  forall g p nleft res v,
-  verifyrule g p nleft true res v ->
+  forall g p d res v,
+  verifyrule g p d true res v ->
   res = None \/ res = Some true.
 Proof.
   intros * H.
@@ -1284,9 +1284,9 @@ Inductive same_result_type : bool -> option bool -> bool -> option bool -> Prop 
   .
 
 Lemma verifyrule_nb_change :
-  forall g p nleft nb nb' res v,
-  verifyrule g p nleft nb res v ->
-  exists res', same_result_type nb res nb' res' /\ verifyrule g p nleft nb' res' v.
+  forall g p d nb nb' res v,
+  verifyrule g p d nb res v ->
+  exists res', same_result_type nb res nb' res' /\ verifyrule g p d nb' res' v.
 Proof.
   intros * H.
   generalize dependent nb'.
@@ -1306,12 +1306,12 @@ Proof.
   try match goal with
     [ IHx1: forall _, exists _, _ /\ verifyrule _ ?p1 _ _ _ _,
       IHx2: forall _, exists _, _ /\ verifyrule _ ?p2 _ _ _ _
-      |- exists res, _ /\ verifyrule ?g (PChoice ?p1 ?p2) ?nleft ?nbx res ?v ] =>
+      |- exists res, _ /\ verifyrule ?g (PChoice ?p1 ?p2) ?d ?nbx res ?v ] =>
           specialize (IHx1 nbx) as [res' [Hsrt1 ?]];
           inversion Hsrt1;
           subst;
           match goal with
-            [ _: verifyrule ?g ?p1 ?nleft ?nbx (Some ?b) _ |- _ ] =>
+            [ _: verifyrule ?g ?p1 ?d ?nbx (Some ?b) _ |- _ ] =>
                 specialize (IHx2 b) as [res'' [Hsrt2 ?]];
                 inversion Hsrt2;
                 subst;
@@ -1321,9 +1321,9 @@ Proof.
 Qed.
 
 Lemma verifyrule_nb_change_none :
-  forall g p nleft nb nb' v,
-  verifyrule g p nleft nb None v ->
-  verifyrule g p nleft nb' None v.
+  forall g p d nb nb' v,
+  verifyrule g p d nb None v ->
+  verifyrule g p d nb' None v.
 Proof.
   intros * H.
   eapply verifyrule_nb_change with (nb' := nb') in H as [res' [Hsrt H]].
@@ -1332,9 +1332,9 @@ Proof.
 Qed.
 
 Lemma verifyrule_nb_change_some :
-  forall g p nleft nb nb' b v,
-  verifyrule g p nleft nb (Some b) v ->
-  exists b', verifyrule g p nleft nb' (Some b') v.
+  forall g p d nb nb' b v,
+  verifyrule g p d nb (Some b) v ->
+  exists b', verifyrule g p d nb' (Some b') v.
 Proof.
   intros * H.
   eapply verifyrule_nb_change with (nb' := nb') in H as [res' [Hsrt H]].
@@ -1344,16 +1344,16 @@ Qed.
 
 Ltac pose_verifyrule_nb_none :=
   try match goal with
-    [ Hx1: verifyrule ?g ?p ?nleft _ None ?v,
-      Hx2: verifyrule ?g ?p ?nleft ?nb _ _ |- _ ] =>
-          assert (verifyrule g p nleft nb None v)
+    [ Hx1: verifyrule ?g ?p ?d _ None ?v,
+      Hx2: verifyrule ?g ?p ?d ?nb _ _ |- _ ] =>
+          assert (verifyrule g p d nb None v)
           by eauto using verifyrule_nb_change_none
   end.
 
 Lemma verifyrule_v_independent_from_nb :
-  forall g p nleft nb nb' res res' v v',
-  verifyrule g p nleft nb res v ->
-  verifyrule g p nleft nb' res' v' ->
+  forall g p d nb nb' res res' v v',
+  verifyrule g p d nb res v ->
+  verifyrule g p d nb' res' v' ->
   v = v'.
 Proof.
   intros * H H'.
@@ -1373,9 +1373,9 @@ Proof.
 Qed.
 
 Lemma verifyrule_nullable_approx :
-  forall g p s nleft nb res v,
+  forall g p s d nb res v,
   matches g p s (Success s) ->
-  verifyrule g p nleft nb res v ->
+  verifyrule g p d nb res v ->
   res = None \/ res = Some true.
 Proof.
   intros * Hm Hv.
@@ -1383,7 +1383,7 @@ Proof.
   generalize dependent v.
   generalize dependent res.
   generalize dependent nb.
-  generalize dependent nleft.
+  generalize dependent d.
   induction Hm; intros;
   inversion Hv; subst;
   try destruct1;
@@ -1402,7 +1402,7 @@ Proof.
   try eq_nth_error;
   eauto using verifyrule_res_none_or_some_true;
   try match goal with
-  [ IHx: _ -> forall nleft nb res v, verifyrule ?g ?p nleft nb res v -> _,
+  [ IHx: _ -> forall d nb res v, verifyrule ?g ?p d nb res v -> _,
     Hx: verifyrule ?g ?p _ _ _ _ |- _ ] =>
       apply IHx in Hx; auto;
       destruct Hx; try discriminate; try destruct1;
@@ -1412,9 +1412,9 @@ Proof.
 Qed.
 
 Theorem verifyrule_fast_forward_exists :
-  forall g p nleft nb res v1 i v2,
-  verifyrule g p nleft nb res (v1 ++ i :: v2) ->
-  exists nleft' nb' res', verifyrule g (PNT i) nleft' nb' res' (i :: v2).
+  forall g p d nb res v1 i v2,
+  verifyrule g p d nb res (v1 ++ i :: v2) ->
+  exists d' nb' res', verifyrule g (PNT i) d' nb' res' (i :: v2).
 Proof.
   intros * H.
   remember (v1 ++ i :: v2) as v.
@@ -1433,13 +1433,13 @@ Proof.
 Qed.
 
 Theorem verifyrule_fast_forward_none_exists :
-  forall g p nleft nb v1 i v2,
-  verifyrule g p nleft nb None (v1 ++ i :: v2) ->
-  exists nleft' nb', verifyrule g (PNT i) nleft' nb' None (i :: v2).
+  forall g p d nb v1 i v2,
+  verifyrule g p d nb None (v1 ++ i :: v2) ->
+  exists d' nb', verifyrule g (PNT i) d' nb' None (i :: v2).
 Proof.
   intros * H.
-  assert (exists nleft' nb' res', verifyrule g (PNT i) nleft' nb' res' (i :: v2))
-  as [nleft' [nb' [res' ?]]]
+  assert (exists d' nb' res', verifyrule g (PNT i) d' nb' res' (i :: v2))
+  as [d' [nb' [res' ?]]]
   by eauto using verifyrule_fast_forward_exists.
   destruct res' as [b|]; eauto;
   remember (v1 ++ i :: v2) as v;
@@ -1447,7 +1447,7 @@ Proof.
   generalize dependent i;
   generalize dependent v1;
   generalize dependent nb';
-  generalize dependent nleft';
+  generalize dependent d';
   generalize dependent b;
   remember None as res;
   induction H;
@@ -1461,46 +1461,46 @@ Proof.
 Qed.
 
 Theorem verifyrule_fast_forward_none :
-  forall g p nb nb' nleft v1 i v2,
-  verifyrule g p nleft nb None (v1 ++ i :: v2) ->
+  forall g p nb nb' d v1 i v2,
+  verifyrule g p d nb None (v1 ++ i :: v2) ->
   verifyrule g (PNT i) (1 + length v2) nb' None (i :: v2).
 Proof.
   intros * H.
-  assert (exists nleft' nb', verifyrule g (PNT i) nleft' nb' None (i :: v2))
-  as [nleft' [nb'' ?]]
+  assert (exists d' nb', verifyrule g (PNT i) d' nb' None (i :: v2))
+  as [d' [nb'' ?]]
   by eauto using verifyrule_fast_forward_none_exists.
-  assert (length (i :: v2) = nleft')
-  by eauto using verifyrule_length_v_eq_nleft.
+  assert (length (i :: v2) = d')
+  by eauto using verifyrule_length_v_eq_depth.
   subst.
   simpl in *.
   eauto using verifyrule_nb_change_none.
 Qed.
 
 Theorem verifyrule_replace_end :
-  forall g p nleft nleft' nb nb' v1 i v2 v3,
-  verifyrule g p nleft nb None (v1 ++ i :: v2) ->
-  verifyrule g (PNT i) nleft' nb' None (i :: v3) ->
+  forall g p d d' nb nb' v1 i v2 v3,
+  verifyrule g p d nb None (v1 ++ i :: v2) ->
+  verifyrule g (PNT i) d' nb' None (i :: v3) ->
   length v2 <= length v3 ->
   verifyrule g p (1 + length v1 + length v3) nb None (v1 ++ i :: v3).
 Proof.
   intros * Hvp Hvi Hle.
-  assert (nleft = 1 + length v1 + length v2).
+  assert (d = 1 + length v1 + length v2).
   {
-    apply verifyrule_length_v_eq_nleft in Hvp.
+    apply verifyrule_length_v_eq_depth in Hvp.
     rewrite app_length in Hvp.
     simpl in Hvp.
     lia.
   }
-  subst nleft.
-  assert (nleft' = 1 + length v3).
+  subst d.
+  assert (d' = 1 + length v3).
   {
-    apply verifyrule_length_v_eq_nleft in Hvi.
+    apply verifyrule_length_v_eq_depth in Hvi.
     simpl in Hvi.
     lia.
   }
-  subst nleft'.
+  subst d'.
   assert (1 + length v1 + length v2 <= 1 + length v1 + length v3) by lia.
-  remember (1 + length v1 + length v2) as nleft.
+  remember (1 + length v1 + length v2) as d.
   remember None as res.
   remember (v1 ++ i :: v2) as v.
   generalize dependent v3.
@@ -1513,7 +1513,7 @@ Proof.
   subst;
   try discriminate;
   repeat specialize_eq_refl;
-  eauto using verifyrule, verifyrule_nleft_le_some_determinism.
+  eauto using verifyrule, verifyrule_depth_le_some_determinism.
   - (* PNT i *)
     destruct v1;
     simpl in *;
@@ -1523,9 +1523,9 @@ Proof.
 Qed.
 
 Theorem verifyrule_repetition_in_v :
-  forall g p nleft v1 v2 v3 nb i,
-  verifyrule g p nleft nb None (v1 ++ i :: v2 ++ i :: v3) ->
-  exists nleft', verifyrule g p nleft' nb None (v1 ++ i :: v2 ++ i :: v2 ++ i :: v3).
+  forall g p d v1 v2 v3 nb i,
+  verifyrule g p d nb None (v1 ++ i :: v2 ++ i :: v3) ->
+  exists d', verifyrule g p d' nb None (v1 ++ i :: v2 ++ i :: v2 ++ i :: v3).
 Proof.
   intros * H.
   assert (verifyrule g (PNT i) (1 + length (v2 ++ i :: v3)) false None (i :: v2 ++ i :: v3))
@@ -1569,54 +1569,54 @@ Proof.
   eauto using verifyrule_replace_end.
 Qed.
 
-Theorem verifyrule_convergence_S_nleft :
-  forall g p nleft nb res v,
-  length g < nleft ->
-  verifyrule g p nleft nb res v ->
-  exists v', verifyrule g p (S nleft) nb res v'.
+Theorem verifyrule_convergence_S_depth :
+  forall g p d nb res v,
+  length g < d ->
+  verifyrule g p d nb res v ->
+  exists v', verifyrule g p (S d) nb res v'.
 Proof.
   intros * Hlt Hv.
   destruct res.
   - (* Some b *)
-    eauto using verifyrule_nleft_le_some_determinism.
+    eauto using verifyrule_depth_le_some_determinism.
   - (* None *)
-    assert (length v = nleft)
-    by eauto using verifyrule_length_v_eq_nleft.
-    subst nleft.
+    assert (length v = d)
+    by eauto using verifyrule_length_v_eq_depth.
+    subst d.
     assert (exists i v1 v2 v3, v = v1 ++ i :: v2 ++ i :: v3)
     as [i [v1 [v2 [v3 Heqv]]]]
     by eauto using pigeonhole_principle, verifyrule_i_in_v_lt_length_g.
     subst v.
-    apply verifyrule_repetition_in_v in Hv as [nleft Hv].
-    assert (length (v1 ++ i :: v2 ++ i :: v2 ++ i :: v3) = nleft)
-    by eauto using verifyrule_length_v_eq_nleft.
-    subst nleft.
+    apply verifyrule_repetition_in_v in Hv as [d Hv].
+    assert (length (v1 ++ i :: v2 ++ i :: v2 ++ i :: v3) = d)
+    by eauto using verifyrule_length_v_eq_depth.
+    subst d.
     match goal with
-      [ Hx: verifyrule ?g ?p ?nleft ?nb None _
-        |- exists v, verifyrule ?g ?p ?nleft' ?nb None v ] =>
-            assert (nleft' <= nleft) by (repeat (rewrite app_length; simpl); lia)
+      [ Hx: verifyrule ?g ?p ?d ?nb None _
+        |- exists v, verifyrule ?g ?p ?d' ?nb None v ] =>
+            assert (d' <= d) by (repeat (rewrite app_length; simpl); lia)
     end.
     match goal with
-      [ Hx: verifyrule _ _ ?nleft _ _ _, Hy: _ <= ?nleft |- _ ] =>
-        specialize (verifyrule_nleft_le_coherent_result_type _ _ _ _ _ _ _ Hx Hy) as [? [? [? ?]]]
+      [ Hx: verifyrule _ _ ?d _ _ _, Hy: _ <= ?d |- _ ] =>
+        specialize (verifyrule_depth_le_coherent_result_type _ _ _ _ _ _ _ Hx Hy) as [? [? [? ?]]]
     end.
     match goal with
-      [ Hx: coherent_return_type_after_nleft_increase _ _ |- _ ] =>
+      [ Hx: coherent_return_type_after_depth_increase _ _ |- _ ] =>
           inversion Hx; subst
     end.
     eauto.
 Qed.
 
 Theorem verifyrule_convergence :
-  forall g p nleft nleft' nb res v,
-  length g < nleft ->
-  verifyrule g p nleft nb res v ->
-  nleft <= nleft' ->
-  exists v', verifyrule g p nleft' nb res v'.
+  forall g p d d' nb res v,
+  length g < d ->
+  verifyrule g p d nb res v ->
+  d <= d' ->
+  exists v', verifyrule g p d' nb res v'.
 Proof.
   intros * Hlt Hv Hle.
-  induction Hle as [|nleft' Hle [v' IH]];
-  eauto using verifyrule_convergence_S_nleft, Nat.lt_le_trans.
+  induction Hle as [|d' Hle [v' IH]];
+  eauto using verifyrule_convergence_S_depth, Nat.lt_le_trans.
 Qed.
 
 Ltac specialize_coherent :=
@@ -1628,9 +1628,9 @@ Ltac specialize_coherent :=
 Lemma verifyrule_safe_grammar_yields_safe_pattern :
   forall g p nb,
   (forall r, In r g -> coherent g r true) ->
-  (forall r nb, In r g -> exists nleft b v, verifyrule g r nleft nb (Some b) v) ->
+  (forall r nb, In r g -> exists d b v, verifyrule g r d nb (Some b) v) ->
   coherent g p true ->
-  exists nleft b v, verifyrule g p nleft nb (Some b) v.
+  exists d b v, verifyrule g p d nb (Some b) v.
 Proof.
   intros * Hgc Hgv Hpc.
   generalize dependent nb.
@@ -1645,14 +1645,14 @@ Proof.
       |- exists _ _ _, verifyrule ?g (_ ?p1 ?p2) _ ?nb _ _ ] =>
           specialize (Hx1 false);
           specialize (Hx2 nb);
-          destruct Hx1 as [nleft1 [b1 [v1 ?]]];
-          destruct Hx2 as [nleft2 [b2 [v2 ?]]];
-          assert (nleft1 <= nleft1 + nleft2) by lia;
-          assert (nleft2 <= nleft1 + nleft2) by lia;
-          assert (verifyrule g p1 (nleft1 + nleft2) false (Some b1) v1)
-          by eauto using verifyrule_nleft_le_some_determinism;
-          assert (verifyrule g p2 (nleft1 + nleft2) nb (Some b2) v2)
-          by eauto using verifyrule_nleft_le_some_determinism;
+          destruct Hx1 as [d1 [b1 [v1 ?]]];
+          destruct Hx2 as [d2 [b2 [v2 ?]]];
+          assert (d1 <= d1 + d2) by lia;
+          assert (d2 <= d1 + d2) by lia;
+          assert (verifyrule g p1 (d1 + d2) false (Some b1) v1)
+          by eauto using verifyrule_depth_le_some_determinism;
+          assert (verifyrule g p2 (d1 + d2) nb (Some b2) v2)
+          by eauto using verifyrule_depth_le_some_determinism;
           destruct b1;
           eauto using verifyrule;
           fail
@@ -1662,15 +1662,15 @@ Proof.
       Hx2: forall nb, exists _ _ _, verifyrule ?g ?p2 _ nb (Some _) _
       |- exists _ _ _, verifyrule ?g (_ ?p1 ?p2) _ ?nb _ _ ] =>
           specialize (Hx1 nb);
-          destruct Hx1 as [nleft1 [b1 [v1 ?]]];
+          destruct Hx1 as [d1 [b1 [v1 ?]]];
           specialize (Hx2 b1);
-          destruct Hx2 as [nleft2 [b2 [v2 ?]]];
-          assert (nleft1 <= nleft1 + nleft2) by lia;
-          assert (nleft2 <= nleft1 + nleft2) by lia;
-          assert (verifyrule g p1 (nleft1 + nleft2) nb (Some b1) v1)
-          by eauto using verifyrule_nleft_le_some_determinism;
-          assert (verifyrule g p2 (nleft1 + nleft2) b1 (Some b2) v2)
-          by eauto using verifyrule_nleft_le_some_determinism;
+          destruct Hx2 as [d2 [b2 [v2 ?]]];
+          assert (d1 <= d1 + d2) by lia;
+          assert (d2 <= d1 + d2) by lia;
+          assert (verifyrule g p1 (d1 + d2) nb (Some b1) v1)
+          by eauto using verifyrule_depth_le_some_determinism;
+          assert (verifyrule g p2 (d1 + d2) b1 (Some b2) v2)
+          by eauto using verifyrule_depth_le_some_determinism;
           destruct b1;
           eauto using verifyrule;
           fail
@@ -1688,37 +1688,37 @@ Proof.
       |- exists _ _ _, verifyrule g (PNT ?n) _ ?nb _ _ ] =>
         assert (In p g) by eauto using nth_error_In;
         assert (coherent g p true) by eauto;
-        assert (exists nleft b v, verifyrule g p nleft nb (Some b) v)
-        as [nleft [b [v ?]]] by eauto;
+        assert (exists d b v, verifyrule g p d nb (Some b) v)
+        as [d [b [v ?]]] by eauto;
         eauto using verifyrule
   end.
 Qed.
 
 (** VerifyRule function with gas **)
 
-Fixpoint verifyrule_comp g p nleft nb gas {struct gas} :=
+Fixpoint verifyrule_comp g p d nb gas {struct gas} :=
   match gas with
   | O => None
   | S gas' => match p with
               | PEmpty => Some (Some true, nil)
               | PChar _ => Some (Some nb, nil)
               | PAnyChar => Some (Some nb, nil)
-              | PSequence p1 p2 => match verifyrule_comp g p1 nleft false gas' with
-                                   | Some (Some true, _) => verifyrule_comp g p2 nleft nb gas'
+              | PSequence p1 p2 => match verifyrule_comp g p1 d false gas' with
+                                   | Some (Some true, _) => verifyrule_comp g p2 d nb gas'
                                    | Some (Some false, v) => Some (Some nb, v)
                                    | res => res
                                    end
-              | PChoice p1 p2 => match verifyrule_comp g p1 nleft nb gas' with
-                                 | Some (Some nb', _) => verifyrule_comp g p2 nleft nb' gas'
+              | PChoice p1 p2 => match verifyrule_comp g p1 d nb gas' with
+                                 | Some (Some nb', _) => verifyrule_comp g p2 d nb' gas'
                                  | res => res
                                  end
-              | PRepetition p' => verifyrule_comp g p' nleft true gas'
-              | PNot p' => verifyrule_comp g p' nleft true gas'
+              | PRepetition p' => verifyrule_comp g p' d true gas'
+              | PNot p' => verifyrule_comp g p' d true gas'
               | PNT i => match nth_error g i with
                          | None => None
-                         | Some p' => match nleft with
+                         | Some p' => match d with
                                       | O => Some (None, nil)
-                                      | S nleft' => match verifyrule_comp g p' nleft' nb gas' with
+                                      | S d' => match verifyrule_comp g p' d' nb gas' with
                                                     | Some (res, v) => Some (res, i :: v)
                                                     | None => None
                                                     end
@@ -1728,15 +1728,15 @@ Fixpoint verifyrule_comp g p nleft nb gas {struct gas} :=
   end.
 
 Lemma verifyrule_comp_soundness :
-  forall g p nleft nb gas res v,
-  verifyrule_comp g p nleft nb gas = Some (res, v) ->
-  verifyrule g p nleft nb res v.
+  forall g p d nb gas res v,
+  verifyrule_comp g p d nb gas = Some (res, v) ->
+  verifyrule g p d nb res v.
 Proof.
   intros * H.
   generalize dependent v.
   generalize dependent res.
   generalize dependent nb.
-  generalize dependent nleft.
+  generalize dependent d.
   generalize dependent p.
   generalize dependent g.
   induction gas; intros;
@@ -1750,15 +1750,15 @@ Proof.
         destruct (nth_error g i) eqn:?;
         try discriminate;
         match goal with
-          [ Hx: match ?nleft with | _ => _ end = _ |- _ ] =>
-              destruct nleft eqn:?;
+          [ Hx: match ?d with | _ => _ end = _ |- _ ] =>
+              destruct d eqn:?;
               try destruct1;
               eauto using verifyrule
         end
   end;
   try match goal with
-    [ Hx: match verifyrule_comp ?g ?p ?nleft ?nb ?gas with | _ => _ end = _ |- _ ] =>
-        destruct (verifyrule_comp g p nleft nb gas) as [[[[]|]]|] eqn:?;
+    [ Hx: match verifyrule_comp ?g ?p ?d ?nb ?gas with | _ => _ end = _ |- _ ] =>
+        destruct (verifyrule_comp g p d nb gas) as [[[[]|]]|] eqn:?;
         try discriminate;
         try destruct1;
         eauto using verifyrule;
@@ -1767,15 +1767,15 @@ Proof.
 Qed.
 
 Lemma verifyrule_comp_S_gas :
-  forall g p nleft nb res v gas,
-  verifyrule_comp g p nleft nb gas = Some (res, v) ->
-  verifyrule_comp g p nleft nb (S gas) = Some (res, v).
+  forall g p d nb res v gas,
+  verifyrule_comp g p d nb gas = Some (res, v) ->
+  verifyrule_comp g p d nb (S gas) = Some (res, v).
 Proof.
   intros.
   generalize dependent v.
   generalize dependent res.
   generalize dependent nb.
-  generalize dependent nleft.
+  generalize dependent d.
   generalize dependent p.
   generalize dependent g.
   induction gas; intros;
@@ -1790,14 +1790,14 @@ Proof.
       [ |- match nth_error ?g ?i with | _ => _ end = _ ] =>
         destruct (nth_error g i) eqn:?; auto;
         match goal with
-          [ |- match ?nleft with | _ => _ end = _ ] =>
-            destruct nleft; auto
+          [ |- match ?d with | _ => _ end = _ ] =>
+            destruct d; auto
         end
   end;
   try match goal with
-    [ Hx: match verifyrule_comp ?g ?p ?nleft ?nb ?gas with | _ => _ end = _ |- _ ] =>
+    [ Hx: match verifyrule_comp ?g ?p ?d ?nb ?gas with | _ => _ end = _ |- _ ] =>
         let H := fresh in
-        destruct (verifyrule_comp g p nleft nb gas) as [[[[]|]]|] eqn:H;
+        destruct (verifyrule_comp g p d nb gas) as [[[[]|]]|] eqn:H;
         try discriminate;
         try destruct1;
         apply IHgas in H;
@@ -1807,10 +1807,10 @@ Proof.
 Qed.
 
 Lemma verifyrule_comp_le_gas :
-  forall g p nleft nb gas1 gas2 res v,
-  verifyrule_comp g p nleft nb gas1 = Some (res, v) ->
+  forall g p d nb gas1 gas2 res v,
+  verifyrule_comp g p d nb gas1 = Some (res, v) ->
   gas1 <= gas2 ->
-  verifyrule_comp g p nleft nb gas2 = Some (res, v).
+  verifyrule_comp g p d nb gas2 = Some (res, v).
 Proof.
   intros * H Hle.
   induction Hle;
@@ -1818,27 +1818,27 @@ Proof.
 Qed.
 
 Lemma verifyrule_comp_termination :
-  forall g p nleft nb,
+  forall g p d nb,
   (forall r, In r g -> coherent g r true) ->
   coherent g p true ->
   exists gas res v,
-  verifyrule_comp g p nleft nb gas = Some (res, v).
+  verifyrule_comp g p d nb gas = Some (res, v).
 Proof.
   intros * Hgc Hpc.
   generalize dependent nb.
   generalize dependent p.
   generalize dependent g.
-  induction nleft using strong_induction.
+  induction d using strong_induction.
   intros.
   generalize dependent nb.
-  generalize dependent nleft.
+  generalize dependent d.
   generalize dependent g.
   induction p; intros;
   inversion Hpc; subst;
   try (exists 1; simpl; eauto; fail);
   try (
     let H := fresh in
-    assert (exists gas res v, verifyrule_comp g p nleft true gas = Some (res, v))
+    assert (exists gas res v, verifyrule_comp g p d true gas = Some (res, v))
     as [gas [res [v H]]] by auto;
     exists (1 + gas);
     simpl;
@@ -1847,25 +1847,25 @@ Proof.
     fail
   ).
   - (* PSequence p1 p2 *)
-    assert (exists gas res v, verifyrule_comp g p1 nleft false gas = Some (res, v))
+    assert (exists gas res v, verifyrule_comp g p1 d false gas = Some (res, v))
     as [gas1 [res1 [v1 ?]]] by auto.
-    assert (exists gas res v, verifyrule_comp g p2 nleft nb gas = Some (res, v))
+    assert (exists gas res v, verifyrule_comp g p2 d nb gas = Some (res, v))
     as [gas2 [res2 [v2 ?]]] by auto.
     assert (gas1 <= gas1 + gas2) by lia.
     assert (gas2 <= gas1 + gas2) by lia.
-    assert (verifyrule_comp g p2 nleft nb (gas1 + gas2) = Some (res2, v2))
+    assert (verifyrule_comp g p2 d nb (gas1 + gas2) = Some (res2, v2))
     by eauto using verifyrule_comp_le_gas.
     exists (1 + gas1 + gas2).
     simpl.
     let H := fresh in
-    assert (verifyrule_comp g p1 nleft false (gas1 + gas2) = Some (res1, v1))
+    assert (verifyrule_comp g p1 d false (gas1 + gas2) = Some (res1, v1))
     as H by eauto using verifyrule_comp_le_gas;
     rewrite H.
     destruct res1 as [[|]|];
     eauto.
   - (* PChoice p1 p2 *)
     let H := fresh in
-    assert (exists gas res v, verifyrule_comp g p1 nleft nb gas = Some (res, v))
+    assert (exists gas res v, verifyrule_comp g p1 d nb gas = Some (res, v))
     as [gas1 [res1 [v1 H]]] by auto;
     destruct res1 as [nb'|];
     try (
@@ -1875,30 +1875,30 @@ Proof.
       eauto;
       fail
     ).
-    assert (exists gas res v, verifyrule_comp g p2 nleft nb' gas = Some (res, v))
+    assert (exists gas res v, verifyrule_comp g p2 d nb' gas = Some (res, v))
     as [gas2 [res2 [v2 ?]]] by auto.
     assert (gas1 <= gas1 + gas2) by lia.
     assert (gas2 <= gas1 + gas2) by lia.
-    assert (verifyrule_comp g p2 nleft nb' (gas1 + gas2) = Some (res2, v2))
+    assert (verifyrule_comp g p2 d nb' (gas1 + gas2) = Some (res2, v2))
     by eauto using verifyrule_comp_le_gas.
     exists (1 + gas1 + gas2).
     simpl.
     let H := fresh in
-    assert (verifyrule_comp g p1 nleft nb (gas1 + gas2) = Some (Some nb', v1))
+    assert (verifyrule_comp g p1 d nb (gas1 + gas2) = Some (Some nb', v1))
     as H by eauto using verifyrule_comp_le_gas;
     rewrite H.
     eauto.
   - (* PNT n *)
-    destruct nleft.
+    destruct d.
     + (* O *)
       exists 1. simpl.
       match goal with
         [ |- exists _ _, match ?x with | _ => _ end = _ ] =>
           destruct x; try discriminate; eauto
       end.
-    + (* S nleft *)
+    + (* S d *)
       let H := fresh in
-      assert (exists gas res v, verifyrule_comp g p nleft nb gas = Some (res, v))
+      assert (exists gas res v, verifyrule_comp g p d nb gas = Some (res, v))
       as [gas [res [v H]]] by eauto using nth_error_In;
       exists (1 + gas);
       simpl;
@@ -1911,22 +1911,22 @@ Proof.
 Qed.
 
 Lemma verifyrule_comp_gas_bounded :
-  forall g p gas nleft nb,
+  forall g p gas d nb,
   (forall r, In r g -> coherent g r true) ->
   coherent g p true ->
-  gas >= pat_size p + nleft * (grammar_size g) ->
+  gas >= pat_size p + d * (grammar_size g) ->
   exists res v,
-  verifyrule_comp g p nleft nb gas = Some (res, v).
+  verifyrule_comp g p d nb gas = Some (res, v).
 Proof.
   intros * Hgc Hpc Hge.
   generalize dependent nb.
   generalize dependent gas.
   generalize dependent p.
   generalize dependent g.
-  induction nleft using strong_induction.
+  induction d using strong_induction.
   intros.
   generalize dependent nb.
-  generalize dependent nleft.
+  generalize dependent d.
   generalize dependent gas.
   generalize dependent g.
   induction p; intros;
@@ -1938,26 +1938,26 @@ Proof.
         inversion Hx
   end;
   try match goal with
-    [ |- exists _ _, _ ?g (_ ?p) ?nleft _ (S ?gas) = _ ] =>
-        assert (gas >= pat_size p + nleft * grammar_size g) by lia
+    [ |- exists _ _, _ ?g (_ ?p) ?d _ (S ?gas) = _ ] =>
+        assert (gas >= pat_size p + d * grammar_size g) by lia
   end;
   try match goal with
-    [ |- exists _ _, _ ?g (_ ?p _) ?nleft _ (S ?gas) = _ ] =>
-        assert (gas >= pat_size p + nleft * grammar_size g) by lia
+    [ |- exists _ _, _ ?g (_ ?p _) ?d _ (S ?gas) = _ ] =>
+        assert (gas >= pat_size p + d * grammar_size g) by lia
   end;
   simpl;
   eauto.
   - (* PSequence p1 p2 *)
-    assert (exists res v, verifyrule_comp g p1 nleft false gas = Some (res, v))
+    assert (exists res v, verifyrule_comp g p1 d false gas = Some (res, v))
     as [res1 [? Hvrp1]] by eauto.
-    assert (exists res v, verifyrule_comp g p2 nleft nb gas = Some (res, v))
+    assert (exists res v, verifyrule_comp g p2 d nb gas = Some (res, v))
     as [? [? ?]] by eauto.
     rewrite Hvrp1.
     destruct res1 as [[|]|]; eauto.
   - (* PChoice p1 p2 *)
-    assert (exists res v, verifyrule_comp g p1 nleft nb gas = Some (res, v))
+    assert (exists res v, verifyrule_comp g p1 d nb gas = Some (res, v))
     as [res1 [? Hvrp1]] by eauto.
-    assert (exists res v, verifyrule_comp g p2 nleft nb gas = Some (res, v))
+    assert (exists res v, verifyrule_comp g p2 d nb gas = Some (res, v))
     as [? [? ?]] by eauto.
     rewrite Hvrp1.
     destruct res1; eauto.
@@ -1966,11 +1966,11 @@ Proof.
       [ Hx: nth_error _ _ = Some _ |- _ ] =>
           rewrite Hx
     end.
-    destruct nleft; eauto.
+    destruct d; eauto.
     assert (pat_size p <= grammar_size g)
     by eauto using nth_error_In, pat_size_le_grammar_size.
-    assert (gas >= pat_size p + nleft * grammar_size g) by lia.
-    assert (exists res v, verifyrule_comp g p nleft nb gas = Some (res, v))
+    assert (gas >= pat_size p + d * grammar_size g) by lia.
+    assert (exists res v, verifyrule_comp g p d nb gas = Some (res, v))
     as [? [? Hvrp]] by eauto using nth_error_In.
     rewrite Hvrp.
     eauto.
@@ -1981,64 +1981,64 @@ Qed.
 
 Inductive nullable : grammar -> pat -> nat -> option bool -> Prop :=
   | NEmpty :
-      forall g nleft,
-      nullable g PEmpty nleft (Some true)
+      forall g d,
+      nullable g PEmpty d (Some true)
   | NChar :
-      forall g a nleft,
-      nullable g (PChar a) nleft (Some false)
+      forall g a d,
+      nullable g (PChar a) d (Some false)
   | NAnyChar :
-      forall g nleft,
-      nullable g PAnyChar nleft (Some false)
+      forall g d,
+      nullable g PAnyChar d (Some false)
   | NSequenceNone :
-      forall g p1 p2 nleft,
-      nullable g p1 nleft None ->
-      nullable g (PSequence p1 p2) nleft None
+      forall g p1 p2 d,
+      nullable g p1 d None ->
+      nullable g (PSequence p1 p2) d None
   | NSequenceSomeFalse :
-      forall g p1 p2 nleft,
-      nullable g p1 nleft (Some false) ->
-      nullable g (PSequence p1 p2) nleft (Some false)
+      forall g p1 p2 d,
+      nullable g p1 d (Some false) ->
+      nullable g (PSequence p1 p2) d (Some false)
   | NSequenceSomeTrue :
-      forall g p1 p2 nleft res,
-      nullable g p1 nleft (Some true) ->
-      nullable g p2 nleft res ->
-      nullable g (PSequence p1 p2) nleft res
+      forall g p1 p2 d res,
+      nullable g p1 d (Some true) ->
+      nullable g p2 d res ->
+      nullable g (PSequence p1 p2) d res
   | NChoiceNone :
-      forall g p1 p2 nleft,
-      nullable g p1 nleft None ->
-      nullable g (PChoice p1 p2) nleft None
+      forall g p1 p2 d,
+      nullable g p1 d None ->
+      nullable g (PChoice p1 p2) d None
   | NChoiceSomeFalse :
-      forall g p1 p2 nleft res,
-      nullable g p1 nleft (Some false) ->
-      nullable g p2 nleft res ->
-      nullable g (PChoice p1 p2) nleft res
+      forall g p1 p2 d res,
+      nullable g p1 d (Some false) ->
+      nullable g p2 d res ->
+      nullable g (PChoice p1 p2) d res
   | NChoiceSomeTrue :
-      forall g p1 p2 nleft,
-      nullable g p1 nleft (Some true) ->
-      nullable g (PChoice p1 p2) nleft (Some true)
+      forall g p1 p2 d,
+      nullable g p1 d (Some true) ->
+      nullable g (PChoice p1 p2) d (Some true)
   | NRepetition :
-      forall g p nleft,
-      nullable g (PRepetition p) nleft (Some true)
+      forall g p d,
+      nullable g (PRepetition p) d (Some true)
   | NNot :
-      forall g p nleft,
-      nullable g (PNot p) nleft (Some true)
+      forall g p d,
+      nullable g (PNot p) d (Some true)
   | NNTZero :
       forall g i p,
       nth_error g i = Some p ->
       nullable g (PNT i) O None
   | NNTSucc :
-      forall g i p res nleft,
+      forall g i p res d,
       nth_error g i = Some p ->
-      nullable g p nleft res ->
-      nullable g (PNT i) (S nleft) res
+      nullable g p d res ->
+      nullable g (PNT i) (S d) res
   .
 
 (* ! {A <- A} |= A *)
 Example nullable_ex1 :
-  forall nleft b,
+  forall d b,
     ~ nullable
     [PNT 0]
     (PNT 0)
-    nleft
+    d
     (Some b).
 Proof.
   intros * H.
@@ -2055,8 +2055,8 @@ Qed.
 
 (* G |= ε *)
 Example nullable_ex2 :
-  forall g nleft,
-  nullable g PEmpty nleft (Some true).
+  forall g d,
+  nullable g PEmpty d (Some true).
 Proof.
   intros.
   eauto using nullable.
@@ -2064,8 +2064,8 @@ Qed.
 
 (* ! G |= 'a' *)
 Example nullable_ex3 :
-  forall g a nleft,
-  nullable g (PChar a) nleft (Some false).
+  forall g a d,
+  nullable g (PChar a) d (Some false).
 Proof.
   intros.
   eauto using nullable.
@@ -2073,8 +2073,8 @@ Qed.
 
 (* ! G |= . *)
 Example nullable_ex4 :
-  forall g nleft,
-  nullable g PAnyChar nleft (Some false).
+  forall g d,
+  nullable g PAnyChar d (Some false).
 Proof.
   intros.
   eauto using nullable.
@@ -2082,8 +2082,8 @@ Qed.
 
 (* G |= ε ε *)
 Example nullable_ex5 :
-  forall g nleft,
-  nullable g (PSequence PEmpty PEmpty) nleft (Some true).
+  forall g d,
+  nullable g (PSequence PEmpty PEmpty) d (Some true).
 Proof.
   intros.
   eauto using nullable.
@@ -2091,8 +2091,8 @@ Qed.
 
 (* ! G |= . ε *)
 Example nullable_ex6 :
-  forall g nleft,
-  nullable g (PSequence PAnyChar PEmpty) nleft (Some false).
+  forall g d,
+  nullable g (PSequence PAnyChar PEmpty) d (Some false).
 Proof.
   intros.
   eauto using nullable.
@@ -2100,8 +2100,8 @@ Qed.
 
 (* ! G |= ε . *)
 Example nullable_ex7 :
-  forall g nleft,
-  nullable g (PSequence PEmpty PAnyChar) nleft (Some false).
+  forall g d,
+  nullable g (PSequence PEmpty PAnyChar) d (Some false).
 Proof.
   intros.
   eauto using nullable.
@@ -2109,8 +2109,8 @@ Qed.
 
 (* ! G |= . . *)
 Example nullable_ex8 :
-  forall g nleft,
-  nullable g (PSequence PAnyChar PAnyChar) nleft (Some false).
+  forall g d,
+  nullable g (PSequence PAnyChar PAnyChar) d (Some false).
 Proof.
   intros.
   eauto using nullable.
@@ -2118,8 +2118,8 @@ Qed.
 
 (* G |= ε / ε *)
 Example nullable_ex9 :
-  forall g nleft,
-  nullable g (PChoice PEmpty PEmpty) nleft (Some true).
+  forall g d,
+  nullable g (PChoice PEmpty PEmpty) d (Some true).
 Proof.
   intros.
   eauto using nullable.
@@ -2127,8 +2127,8 @@ Qed.
 
 (* G |= . / ε *)
 Example nullable_ex10 :
-  forall g nleft,
-  nullable g (PChoice PAnyChar PEmpty) nleft (Some true).
+  forall g d,
+  nullable g (PChoice PAnyChar PEmpty) d (Some true).
 Proof.
   intros.
   eauto using nullable.
@@ -2136,8 +2136,8 @@ Qed.
 
 (* G |= ε / . *)
 Example nullable_ex11 :
-  forall g nleft,
-  nullable g (PChoice PEmpty PAnyChar) nleft (Some true).
+  forall g d,
+  nullable g (PChoice PEmpty PAnyChar) d (Some true).
 Proof.
   intros.
   eauto using nullable.
@@ -2145,8 +2145,8 @@ Qed.
 
 (* ! G |= . / . *)
 Example nullable_ex12 :
-  forall g nleft,
-  nullable g (PChoice PAnyChar PAnyChar) nleft (Some false).
+  forall g d,
+  nullable g (PChoice PAnyChar PAnyChar) d (Some false).
 Proof.
   intros.
   eauto using nullable.
@@ -2154,8 +2154,8 @@ Qed.
 
 (* G |= p* *)
 Example nullable_ex13 :
-  forall g p nleft,
-  nullable g (PRepetition p) nleft (Some true).
+  forall g p d,
+  nullable g (PRepetition p) d (Some true).
 Proof.
   intros.
   eauto using nullable.
@@ -2163,8 +2163,8 @@ Qed.
 
 (* G |= !p *)
 Example nullable_ex14 :
-  forall g p nleft,
-  nullable g (PNot p) nleft (Some true).
+  forall g p d,
+  nullable g (PNot p) d (Some true).
 Proof.
   intros.
   eauto using nullable.
@@ -2172,11 +2172,11 @@ Qed.
 
 (* ! { P <- . P } |= P *)
 Example nullable_ex15 :
-  forall nleft,
+  forall d,
   nullable
     [PSequence PAnyChar (PNT 0)]
     (PNT 0)
-    (S nleft)
+    (S d)
     (Some false).
 Proof.
   intros.
@@ -2186,11 +2186,11 @@ Qed.
 
 (* { P <- . P / ε } |= P *)
 Example nullable_ex16 :
-  forall nleft,
+  forall d,
   nullable
     [PChoice (PSequence PAnyChar (PNT 0)) PEmpty]
     (PNT 0)
-    (S nleft)
+    (S d)
     (Some true).
 Proof.
   intros.
@@ -2200,8 +2200,8 @@ Qed.
 
 (* ! {} |= A *)
 Example nullable_ex17 :
-  forall nleft res,
-  ~ nullable [] (PNT 0) nleft res.
+  forall d res,
+  ~ nullable [] (PNT 0) d res.
 Proof.
   intros * H.
   inversion H;
@@ -2211,11 +2211,11 @@ Qed.
 
 (* { A <- 'a' A | ε ; B <- A A } |= A B *)
 Example nullable_ex18 :
-  forall nleft,
+  forall d,
   nullable
   [PChoice (PSequence (PChar "a") (PNT 0)) PEmpty; PSequence (PNT 0) (PNT 0)]
   (PSequence (PNT 0) (PNT 1))
-  (S (S nleft))
+  (S (S d))
   (Some true).
 Proof.
   intros.
@@ -2228,9 +2228,9 @@ Proof.
 Qed.
 
 Lemma nullable_determinism :
-  forall g p nleft res1 res2,
-  nullable g p nleft res1 ->
-  nullable g p nleft res2 ->
+  forall g p d res1 res2,
+  nullable g p d res1 ->
+  nullable g p d res2 ->
   res1 = res2.
 Proof.
   intros * H1 H2.
@@ -2240,8 +2240,8 @@ Proof.
   inversion H2; subst;
   try eq_nth_error;
   try match goal with
-  [ IHx: forall resx, nullable ?g ?p ?nleft resx -> ?res1 = resx,
-    Hx: nullable ?g ?p ?nleft ?res2 |- _ ] =>
+  [ IHx: forall resx, nullable ?g ?p ?d resx -> ?res1 = resx,
+    Hx: nullable ?g ?p ?d ?res2 |- _ ] =>
         apply IHx in Hx;
         discriminate
   end;
@@ -2250,17 +2250,17 @@ Qed.
 
 Ltac pose_nullable_determinism :=
   match goal with
-    [ Hx1: nullable ?g ?p ?nleft ?res1,
-      Hx2: nullable ?g ?p ?nleft ?res2 |- _ ] =>
+    [ Hx1: nullable ?g ?p ?d ?res1,
+      Hx2: nullable ?g ?p ?d ?res2 |- _ ] =>
           assert (res1 = res2)
           by eauto using nullable_determinism;
           clear Hx2
   end.
 
-Lemma nullable_Some_S_nleft :
-  forall g p nleft b,
-  nullable g p nleft (Some b) ->
-  nullable g p (S nleft) (Some b).
+Lemma nullable_Some_S_depth :
+  forall g p d b,
+  nullable g p d (Some b) ->
+  nullable g p (S d) (Some b).
 Proof.
   intros * H.
   remember (Some b) as res.
@@ -2270,21 +2270,21 @@ Proof.
   eauto using nullable.
 Qed.
 
-Lemma nullable_Some_nleft_le :
-  forall g p nleft nleft' b,
-  nullable g p nleft (Some b) ->
-  nleft <= nleft' ->
-  nullable g p nleft' (Some b).
+Lemma nullable_Some_depth_le :
+  forall g p d d' b,
+  nullable g p d (Some b) ->
+  d <= d' ->
+  nullable g p d' (Some b).
 Proof.
   intros * H Hle.
   induction Hle;
-  eauto using nullable_Some_S_nleft.
+  eauto using nullable_Some_S_depth.
 Qed.
 
 Lemma verifyrule_similar_to_nullable :
-  forall g p nleft b v,
-  verifyrule g p nleft false (Some b) v ->
-  nullable g p nleft (Some b).
+  forall g p d b v,
+  verifyrule g p d false (Some b) v ->
+  nullable g p d (Some b).
 Proof.
   intros * H.
   remember (Some b) as res.
@@ -2309,11 +2309,11 @@ Proof.
 Qed.
 
 Lemma nullable_none_is_verifyrule_none :
-  forall g p nleft,
+  forall g p d,
   (forall r, In r g -> coherent g r true) ->
   coherent g p true ->
-  nullable g p nleft None ->
-  exists v, verifyrule g p nleft false None v.
+  nullable g p d None ->
+  exists v, verifyrule g p d false None v.
 Proof.
   intros * Hcg Hcp Hn.
   remember None as res.
@@ -2339,14 +2339,14 @@ Proof.
   try destruct_exists_hyp;
   eauto using verifyrule;
   try (
-    assert (exists gas res v, verifyrule_comp g p1 nleft false gas = Some (res, v))
+    assert (exists gas res v, verifyrule_comp g p1 d false gas = Some (res, v))
     as [gas [res' [v Hvcp1]]]
     by eauto using verifyrule_comp_termination;
-    assert (verifyrule g p1 nleft false res' v)
+    assert (verifyrule g p1 d false res' v)
     by eauto using verifyrule_comp_soundness;
     destruct res';
     eauto using verifyrule;
-    assert (nullable g p1 nleft (Some b))
+    assert (nullable g p1 d (Some b))
     by eauto using verifyrule_similar_to_nullable;
     pose_nullable_determinism;
     destruct1;
@@ -2365,8 +2365,8 @@ Proof.
 Qed.
 
 Lemma nullable_Some_false_matches :
-  forall g p nleft,
-  nullable g p nleft (Some false) ->
+  forall g p d,
+  nullable g p d (Some false) ->
   ~ exists s, matches g p s (Success s).
 Proof.
   intros * Hnullable [s Hmatches].
@@ -2394,8 +2394,8 @@ Proof.
 Qed.
 
 Lemma nullable_Some_false_proper_suffix :
-  forall g p nleft s s',
-  nullable g p nleft (Some false) ->
+  forall g p d s s',
+  nullable g p d (Some false) ->
   matches g p s (Success s') ->
   proper_suffix s' s.
 Proof.
@@ -2410,42 +2410,42 @@ Proof.
 Qed.
 
 Lemma nullable_convergence :
-  forall g p nleft nleft' res,
+  forall g p d d' res,
   (forall r, In r g -> coherent g r true) ->
-  (forall r nb, In r g -> exists nleft b v, verifyrule g r nleft nb (Some b) v) ->
+  (forall r nb, In r g -> exists d b v, verifyrule g r d nb (Some b) v) ->
   coherent g p true ->
-  length g < nleft ->
-  nullable g p nleft res ->
-  nleft <= nleft' ->
-  nullable g p nleft' res.
+  length g < d ->
+  nullable g p d res ->
+  d <= d' ->
+  nullable g p d' res.
 Proof.
   intros * Hgc Hgv Hpc Hlt H Hle.
-  assert (exists gas res v, verifyrule_comp g p nleft false gas = Some (res, v))
+  assert (exists gas res v, verifyrule_comp g p d false gas = Some (res, v))
   as [? [? [? ?]]]
   by eauto using verifyrule_comp_termination.
   match goal with
-    [ Hx: verifyrule_comp ?g ?p ?nleft false ?gas = Some (?res, ?v) |- _ ] =>
-        assert (verifyrule g p nleft false res v)
+    [ Hx: verifyrule_comp ?g ?p ?d false ?gas = Some (?res, ?v) |- _ ] =>
+        assert (verifyrule g p d false res v)
         by eauto using verifyrule_comp_soundness
   end.
-  assert (exists nleft b v, verifyrule g p nleft false (Some b) v)
+  assert (exists d b v, verifyrule g p d false (Some b) v)
   as [? [? [? ?]]]
   by eauto using verifyrule_safe_grammar_yields_safe_pattern.
   match goal with
-    [ Hx: verifyrule ?g ?p ?nleft1 false (Some ?b) ?v1,
-      Hy: verifyrule ?g ?p ?nleft2 false ?res ?v2,
-      Hz: length ?g < ?nleft2 |- _ ] =>
-          destruct (Compare_dec.le_ge_dec nleft1 nleft2);
+    [ Hx: verifyrule ?g ?p ?d1 false (Some ?b) ?v1,
+      Hy: verifyrule ?g ?p ?d2 false ?res ?v2,
+      Hz: length ?g < ?d2 |- _ ] =>
+          destruct (Compare_dec.le_ge_dec d1 d2);
           try match goal with
-            [ Hw: ?nleft1 <= ?nleft2,
-              Hv: length ?g < ?nleft2 |- _ ] =>
-                  assert (verifyrule g p nleft2 false (Some b) v1)
-                  by eauto using verifyrule_nleft_le_some_determinism
+            [ Hw: ?d1 <= ?d2,
+              Hv: length ?g < ?d2 |- _ ] =>
+                  assert (verifyrule g p d2 false (Some b) v1)
+                  by eauto using verifyrule_depth_le_some_determinism
           end;
           try match goal with
-            [ Hw: ?nleft1 >= ?nleft2 |- _ ] =>
-                assert (nleft2 <= nleft1) by lia;
-                assert (exists v', verifyrule g p nleft1 false res v')
+            [ Hw: ?d1 >= ?d2 |- _ ] =>
+                assert (d2 <= d1) by lia;
+                assert (exists v', verifyrule g p d1 false res v')
                 as [? ?]
                 by eauto using verifyrule_convergence;
                 pose_verifyrule_determinism;
@@ -2453,13 +2453,13 @@ Proof.
           end
   end;
   match goal with
-    [ Hx: nullable ?g ?p ?nleft ?res,
-      Hy: verifyrule ?g ?p ?nleft false (Some ?b) ?v |- _ ] =>
-          assert (nullable g p nleft (Some b))
+    [ Hx: nullable ?g ?p ?d ?res,
+      Hy: verifyrule ?g ?p ?d false (Some ?b) ?v |- _ ] =>
+          assert (nullable g p d (Some b))
           by eauto using verifyrule_similar_to_nullable;
           pose_nullable_determinism;
           subst;
-          assert (exists v', verifyrule g p nleft' false (Some b) v')
+          assert (exists v', verifyrule g p d' false (Some b) v')
           as [? ?]
           by eauto using verifyrule_convergence;
           eauto using verifyrule_similar_to_nullable
@@ -2468,27 +2468,27 @@ Qed.
 
 (** Nullable function with gas **)
 
-Fixpoint nullable_comp g p nleft gas {struct gas} :=
+Fixpoint nullable_comp g p d gas {struct gas} :=
   match gas with
   | O => None
   | S gas' => match p with
               | PEmpty => Some (Some true)
               | PChar _ => Some (Some false)
               | PAnyChar => Some (Some false)
-              | PSequence p1 p2 => match nullable_comp g p1 nleft gas' with
-                                   | Some (Some true) => nullable_comp g p2 nleft gas'
+              | PSequence p1 p2 => match nullable_comp g p1 d gas' with
+                                   | Some (Some true) => nullable_comp g p2 d gas'
                                    | ob => ob
                                    end
-              | PChoice p1 p2 => match nullable_comp g p1 nleft gas' with
-                                 | Some (Some false) => nullable_comp g p2 nleft gas'
+              | PChoice p1 p2 => match nullable_comp g p1 d gas' with
+                                 | Some (Some false) => nullable_comp g p2 d gas'
                                  | ob => ob
                                  end
               | PRepetition _ => Some (Some true)
               | PNot _ => Some (Some true)
               | PNT i => match nth_error g i with
-                         | Some p' => match nleft with
+                         | Some p' => match d with
                                       | O => Some None
-                                      | S nleft' => nullable_comp g p' nleft' gas'
+                                      | S d' => nullable_comp g p' d' gas'
                                       end
                          | None => None
                          end
@@ -2496,13 +2496,13 @@ Fixpoint nullable_comp g p nleft gas {struct gas} :=
   end.
 
 Lemma nullable_comp_soundness :
-  forall g p nleft gas res,
-  nullable_comp g p nleft gas = Some res ->
-  nullable g p nleft res.
+  forall g p d gas res,
+  nullable_comp g p d gas = Some res ->
+  nullable g p d res.
 Proof.
   intros * H.
   generalize dependent res.
-  generalize dependent nleft.
+  generalize dependent d.
   generalize dependent p.
   generalize dependent g.
   induction gas; intros; try discriminate.
@@ -2510,7 +2510,7 @@ Proof.
   try (simpl in H; discriminate; fail);
   try (
     simpl in H;
-    try destruct (nullable_comp g p1 nleft gas)
+    try destruct (nullable_comp g p1 d gas)
     as [[[|]|]|] eqn:?;
     try discriminate;
     try destruct1;
@@ -2522,7 +2522,7 @@ Proof.
     destruct (nth_error g n) eqn:?;
     try discriminate;
     try destruct1;
-    destruct nleft;
+    destruct d;
     try discriminate;
     try destruct1;
     assert (In p g) as HIn by (eauto using nth_error_In);
@@ -2544,13 +2544,13 @@ Ltac destruct_match_subject_in_hyp :=
   end.
 
 Lemma nullable_comp_S_gas :
-  forall g p nleft gas res,
-  nullable_comp g p nleft gas = Some res ->
-  nullable_comp g p nleft (S gas) = Some res.
+  forall g p d gas res,
+  nullable_comp g p d gas = Some res ->
+  nullable_comp g p d (S gas) = Some res.
 Proof.
   intros * H.
   generalize dependent res.
-  generalize dependent nleft.
+  generalize dependent d.
   generalize dependent p.
   generalize dependent g.
   induction gas; intros; try discriminate;
@@ -2558,8 +2558,8 @@ Proof.
   try destruct1;
   auto;
   try (
-    destruct (nullable_comp g p1 nleft gas) as [[[|]|]|] eqn:Hn1;
-    destruct (nullable_comp g p2 nleft gas) as [[[|]|]|] eqn:Hn2;
+    destruct (nullable_comp g p1 d gas) as [[[|]|]|] eqn:Hn1;
+    destruct (nullable_comp g p2 d gas) as [[[|]|]|] eqn:Hn2;
     try discriminate;
     destruct1;
     try apply IHgas in Hn1;
@@ -2585,10 +2585,10 @@ Proof.
 Qed.
 
 Lemma nullable_comp_le_gas :
-  forall g p nleft gas1 gas2 res,
-  nullable_comp g p nleft gas1 = Some res ->
+  forall g p d gas1 gas2 res,
+  nullable_comp g p d gas1 = Some res ->
   gas1 <= gas2 ->
-  nullable_comp g p nleft gas2 = Some res.
+  nullable_comp g p d gas2 = Some res.
 Proof.
   intros * H Hle.
   induction Hle;
@@ -2599,14 +2599,14 @@ Qed.
    instead of summing up the pat_size of each rule of the grammar,
    but the sum makes the proof of lower bound easier *)
 Lemma nullable_comp_gas_bounded :
-  forall g p nleft gas,
+  forall g p d gas,
   (forall r, In r g -> coherent g r true) ->
   coherent g p true ->
-  gas >= pat_size p + nleft * (grammar_size g) ->
-  exists res, nullable_comp g p nleft gas = Some res.
+  gas >= pat_size p + d * (grammar_size g) ->
+  exists res, nullable_comp g p d gas = Some res.
 Proof.
   intros * Hgc Hpc Hge.
-  generalize dependent nleft.
+  generalize dependent d.
   generalize dependent p.
   generalize dependent g.
   induction gas; intros;
@@ -2616,10 +2616,10 @@ Proof.
   try (simpl; eauto; fail);
   try (
     simpl in Hge;
-    assert (gas >= pat_size p1 + nleft * grammar_size g) by lia;
-    assert (gas >= pat_size p2 + nleft * grammar_size g) by lia;
-    assert (exists res, nullable_comp g p1 nleft gas = Some res) as [res1 Hn1] by auto;
-    assert (exists res, nullable_comp g p2 nleft gas = Some res) by auto;
+    assert (gas >= pat_size p1 + d * grammar_size g) by lia;
+    assert (gas >= pat_size p2 + d * grammar_size g) by lia;
+    assert (exists res, nullable_comp g p1 d gas = Some res) as [res1 Hn1] by auto;
+    assert (exists res, nullable_comp g p2 d gas = Some res) by auto;
     simpl;
     rewrite Hn1;
     destruct res1 as [[|]|];
@@ -2635,9 +2635,9 @@ Proof.
           rewrite Hx
     end;
     assert (In p g) as HIn by (eauto using nth_error_In);
-    destruct nleft; eauto;
+    destruct d; eauto;
     specialize (pat_size_le_grammar_size _ _ HIn) as Hle;
-    assert (gas >= pat_size p + nleft * grammar_size g) by lia;
+    assert (gas >= pat_size p + d * grammar_size g) by lia;
     auto;
     fail
   ).
@@ -2647,11 +2647,11 @@ Qed.
    We just know there exists SOME gas for which nullable_comp
    gives SOME result. :-) *)
 Lemma nullable_comp_termination :
-  forall g p nleft,
+  forall g p d,
   (forall r, In r g -> coherent g r true) ->
   coherent g p true ->
   exists gas b,
-  nullable_comp g p nleft gas = Some b.
+  nullable_comp g p d gas = Some b.
 Proof.
   eauto using nullable_comp_gas_bounded.
 Qed.
@@ -2661,66 +2661,66 @@ Qed.
 
 Inductive checkloops : grammar -> pat -> nat -> option bool -> Prop :=
   | CLEmpty :
-      forall g nleft,
-      checkloops g PEmpty nleft (Some false)
+      forall g d,
+      checkloops g PEmpty d (Some false)
   | CLChar :
-      forall g a nleft,
-      checkloops g (PChar a) nleft (Some false)
+      forall g a d,
+      checkloops g (PChar a) d (Some false)
   | CLAnyChar :
-      forall g nleft,
-      checkloops g PAnyChar nleft (Some false)
+      forall g d,
+      checkloops g PAnyChar d (Some false)
   | CLSequenceNone :
-      forall g p1 p2 nleft,
-      checkloops g p1 nleft None ->
-      checkloops g (PSequence p1 p2) nleft None
+      forall g p1 p2 d,
+      checkloops g p1 d None ->
+      checkloops g (PSequence p1 p2) d None
   | CLSequenceSomeTrue :
-      forall g p1 p2 nleft,
-      checkloops g p1 nleft (Some true) ->
-      checkloops g (PSequence p1 p2) nleft (Some true)
+      forall g p1 p2 d,
+      checkloops g p1 d (Some true) ->
+      checkloops g (PSequence p1 p2) d (Some true)
   | CLSequenceSomeFalse :
-      forall g p1 p2 res nleft,
-      checkloops g p1 nleft (Some false) ->
-      checkloops g p2 nleft res ->
-      checkloops g (PSequence p1 p2) nleft res
+      forall g p1 p2 res d,
+      checkloops g p1 d (Some false) ->
+      checkloops g p2 d res ->
+      checkloops g (PSequence p1 p2) d res
   | CLChoiceNone :
-      forall g p1 p2 nleft,
-      checkloops g p1 nleft None ->
-      checkloops g (PChoice p1 p2) nleft None
+      forall g p1 p2 d,
+      checkloops g p1 d None ->
+      checkloops g (PChoice p1 p2) d None
   | CLChoiceSomeTrue :
-      forall g p1 p2 nleft,
-      checkloops g p1 nleft (Some true) ->
-      checkloops g (PChoice p1 p2) nleft (Some true)
+      forall g p1 p2 d,
+      checkloops g p1 d (Some true) ->
+      checkloops g (PChoice p1 p2) d (Some true)
   | CLChoiceSomeFalse :
-      forall g p1 p2 nleft res,
-      checkloops g p1 nleft (Some false) ->
-      checkloops g p2 nleft res ->
-      checkloops g (PChoice p1 p2) nleft res
+      forall g p1 p2 d res,
+      checkloops g p1 d (Some false) ->
+      checkloops g p2 d res ->
+      checkloops g (PChoice p1 p2) d res
   | CLRepetitionLR :
-      forall g p nleft,
-      nullable g p nleft None ->
-      checkloops g (PRepetition p) nleft None
+      forall g p d,
+      nullable g p d None ->
+      checkloops g (PRepetition p) d None
   | CLRepetitionNullable :
-      forall g p nleft,
-      nullable g p nleft (Some true) ->
-      checkloops g (PRepetition p) nleft (Some true)
+      forall g p d,
+      nullable g p d (Some true) ->
+      checkloops g (PRepetition p) d (Some true)
   | CLRepetitionNotNullable :
-      forall g p nleft res,
-      nullable g p nleft (Some false) ->
-      checkloops g p nleft res ->
-      checkloops g (PRepetition p) nleft res
+      forall g p d res,
+      nullable g p d (Some false) ->
+      checkloops g p d res ->
+      checkloops g (PRepetition p) d res
   | CLNot :
-      forall g p nleft res,
-      checkloops g p nleft res ->
-      checkloops g (PNot p) nleft res
+      forall g p d res,
+      checkloops g p d res ->
+      checkloops g (PNot p) d res
   | CLNT :
-      forall g i nleft,
-      checkloops g (PNT i) nleft (Some false)
+      forall g i d,
+      checkloops g (PNT i) d (Some false)
   .
 
 Theorem checkloops_determinism :
-  forall g p nleft b1 b2,
-  checkloops g p nleft b1 ->
-  checkloops g p nleft b2 ->
+  forall g p d b1 b2,
+  checkloops g p d b1 ->
+  checkloops g p d b2 ->
   b1 = b2.
 Proof.
   intros * H1 H2.
@@ -2738,17 +2738,17 @@ Qed.
 
 Ltac pose_checkloops_determinism :=
   match goal with
-    [ Hx1: checkloops ?g ?p ?nleft ?res1,
-      Hx2: checkloops ?g ?p ?nleft ?res2 |- _ ] =>
+    [ Hx1: checkloops ?g ?p ?d ?res1,
+      Hx2: checkloops ?g ?p ?d ?res2 |- _ ] =>
           assert (res1 = res2)
           by eauto using checkloops_determinism;
           clear Hx2
   end.
 
-Theorem checkloops_Some_S_nleft :
-  forall g p nleft b,
-  checkloops g p nleft (Some b) ->
-  checkloops g p (S nleft) (Some b).
+Theorem checkloops_Some_S_depth :
+  forall g p d b,
+  checkloops g p d (Some b) ->
+  checkloops g p (S d) (Some b).
 Proof.
   intros * H.
   remember (Some b) as res.
@@ -2757,41 +2757,41 @@ Proof.
   intros;
   try destruct1;
   try discriminate;
-  eauto using checkloops, nullable_Some_S_nleft.
+  eauto using checkloops, nullable_Some_S_depth.
 Qed.
 
-Theorem checkloops_Some_nleft_le :
-  forall g p nleft nleft' b,
-  checkloops g p nleft (Some b) ->
-  nleft <= nleft' ->
-  checkloops g p nleft' (Some b).
+Theorem checkloops_Some_depth_le :
+  forall g p d d' b,
+  checkloops g p d (Some b) ->
+  d <= d' ->
+  checkloops g p d' (Some b).
 Proof.
   intros * H Hle.
   induction Hle;
-  eauto using checkloops_Some_S_nleft.
+  eauto using checkloops_Some_S_depth.
 Qed.
 
 Lemma checkloops_Some_determinism :
-  forall g p nleft1 nleft2 b1 b2,
-  checkloops g p nleft1 (Some b1) ->
-  checkloops g p nleft2 (Some b2) ->
+  forall g p d1 d2 b1 b2,
+  checkloops g p d1 (Some b1) ->
+  checkloops g p d2 (Some b2) ->
   b1 = b2.
 Proof.
   intros * H1 H2.
-  destruct (Compare_dec.le_ge_dec nleft1 nleft2);
+  destruct (Compare_dec.le_ge_dec d1 d2);
   try match goal with
     [ Hge: ?x >= ?y |- _ ] =>
         assert (y <= x) by lia
   end;
   match goal with
-    [ Hx: checkloops ?g ?p ?nleftx (Some ?bx),
-      Hle: ?nleftx <= ?nlefty |- _ ] =>
-          assert (checkloops g p nlefty (Some bx))
-          by eauto using checkloops_Some_nleft_le
+    [ Hx: checkloops ?g ?p ?dx (Some ?bx),
+      Hle: ?dx <= ?dy |- _ ] =>
+          assert (checkloops g p dy (Some bx))
+          by eauto using checkloops_Some_depth_le
   end;
   match goal with
-    [ Hx1: checkloops ?g ?p ?nleft (Some ?b1),
-      Hx2: checkloops ?g ?p ?nleft (Some ?b2) |- _ ] =>
+    [ Hx1: checkloops ?g ?p ?d (Some ?b1),
+      Hx2: checkloops ?g ?p ?d (Some ?b2) |- _ ] =>
           assert (Some b1 = Some b2)
           by eauto using checkloops_determinism
   end;
@@ -2802,9 +2802,9 @@ Qed.
 Lemma checkloops_safe_grammar :
   forall g p,
   (forall r, In r g -> coherent g r true) ->
-  (forall r nb, In r g -> exists nleft b v, verifyrule g r nleft nb (Some b) v) ->
+  (forall r nb, In r g -> exists d b v, verifyrule g r d nb (Some b) v) ->
   coherent g p true ->
-  exists nleft b, checkloops g p nleft (Some b).
+  exists d b, checkloops g p d (Some b).
 Proof.
   intros * Hgc Hgv Hpc.
   induction p;
@@ -2812,41 +2812,41 @@ Proof.
   repeat specialize_coherent;
   repeat destruct_exists_hyp;
   try match goal with
-    [ Hx1: checkloops ?g ?p1 ?nleft1 (Some ?b1),
-      Hx2: checkloops ?g ?p2 ?nleft2 (Some ?b2)
+    [ Hx1: checkloops ?g ?p1 ?d1 (Some ?b1),
+      Hx2: checkloops ?g ?p2 ?d2 (Some ?b2)
       |- exists _ _, checkloops ?g (_ ?p1 ?p2) _ _ ] =>
-          assert (nleft1 <= nleft1 + nleft2) by lia;
-          assert (nleft2 <= nleft1 + nleft2) by lia;
-          assert (checkloops g p1 (nleft1 + nleft2) (Some b1))
-          by eauto using checkloops_Some_nleft_le;
-          assert (checkloops g p2 (nleft1 + nleft2) (Some b2))
-          by eauto using checkloops_Some_nleft_le;
+          assert (d1 <= d1 + d2) by lia;
+          assert (d2 <= d1 + d2) by lia;
+          assert (checkloops g p1 (d1 + d2) (Some b1))
+          by eauto using checkloops_Some_depth_le;
+          assert (checkloops g p2 (d1 + d2) (Some b2))
+          by eauto using checkloops_Some_depth_le;
           destruct b1;
           eauto using checkloops;
           fail
   end;
   try match goal with
     [ Hx: coherent ?g ?p true,
-      Hy: checkloops ?g ?p ?nleft' (Some ?b')
+      Hy: checkloops ?g ?p ?d' (Some ?b')
       |- exists _ _, checkloops ?g (PRepetition ?p) _ _ ] =>
-          assert (exists nleft b v, verifyrule g p nleft false (Some b) v)
-          as [nleft [b [v ?]]] by eauto using verifyrule_safe_grammar_yields_safe_pattern;
-          assert (nullable g p nleft (Some b))
+          assert (exists d b v, verifyrule g p d false (Some b) v)
+          as [d [b [v ?]]] by eauto using verifyrule_safe_grammar_yields_safe_pattern;
+          assert (nullable g p d (Some b))
           by eauto using verifyrule_similar_to_nullable;
-          assert (nleft <= nleft + nleft') by lia;
-          assert (nleft' <= nleft + nleft') by lia;
-          assert (nullable g p (nleft + nleft') (Some b))
-          by eauto using nullable_Some_nleft_le;
-          assert (checkloops g p (nleft + nleft') (Some b'))
-          by eauto using checkloops_Some_nleft_le;
+          assert (d <= d + d') by lia;
+          assert (d' <= d + d') by lia;
+          assert (nullable g p (d + d') (Some b))
+          by eauto using nullable_Some_depth_le;
+          assert (checkloops g p (d + d') (Some b'))
+          by eauto using checkloops_Some_depth_le;
           destruct b;
           eauto using checkloops;
           fail
   end;
   try match goal with
-    [ Hx: checkloops ?g ?p ?nleft (Some _)
+    [ Hx: checkloops ?g ?p ?d (Some _)
       |- exists _ _, checkloops ?g (_ ?p) _ _ ] =>
-          exists nleft;
+          exists d;
           eauto using checkloops;
           fail
   end;
@@ -2854,17 +2854,17 @@ Proof.
 Qed.
 
 Lemma checkloops_convergence :
-  forall g p nleft nleft' res,
+  forall g p d d' res,
   (forall r, In r g -> coherent g r true) ->
-  (forall r nb, In r g -> exists nleft b v, verifyrule g r nleft nb (Some b) v) ->
+  (forall r nb, In r g -> exists d b v, verifyrule g r d nb (Some b) v) ->
   coherent g p true ->
-  length g < nleft ->
-  checkloops g p nleft res ->
-  nleft <= nleft' ->
-  checkloops g p nleft' res.
+  length g < d ->
+  checkloops g p d res ->
+  d <= d' ->
+  checkloops g p d' res.
 Proof.
   intros * Hgc Hgv Hpc Hlt Hcl Hle.
-  generalize dependent nleft'.
+  generalize dependent d'.
   induction Hcl;
   intros;
   inversion Hpc; subst;
@@ -2872,24 +2872,24 @@ Proof.
 Qed.
 
 Lemma checkloops_Some_convergence :
-  forall g p nleft nleft' b res,
+  forall g p d d' b res,
   (forall r, In r g -> coherent g r true) ->
-  (forall r nb, In r g -> exists nleft b v, verifyrule g r nleft nb (Some b) v) ->
+  (forall r nb, In r g -> exists d b v, verifyrule g r d nb (Some b) v) ->
   coherent g p true ->
-  checkloops g p nleft (Some b) ->
-  length g < nleft' ->
-  checkloops g p nleft' res ->
+  checkloops g p d (Some b) ->
+  length g < d' ->
+  checkloops g p d' res ->
   res = Some b.
 Proof.
   intros * Hgc Hgv Hpc Hc Hlt Hc'.
-  destruct (Compare_dec.le_ge_dec nleft nleft');
+  destruct (Compare_dec.le_ge_dec d d');
   match goal with
-  | [ _: ?nleft <= ?nleft' |- _ ] =>
-      assert (checkloops g p nleft' (Some b))
-      by eauto using checkloops_Some_nleft_le
-  | [ _: ?nleft >= ?nleft' |- _ ] =>
-      assert (nleft' <= nleft) by lia;
-      assert (checkloops g p nleft res)
+  | [ _: ?d <= ?d' |- _ ] =>
+      assert (checkloops g p d' (Some b))
+      by eauto using checkloops_Some_depth_le
+  | [ _: ?d >= ?d' |- _ ] =>
+      assert (d' <= d) by lia;
+      assert (checkloops g p d res)
       by eauto using checkloops_convergence
   end;
   pose_checkloops_determinism;
@@ -2899,38 +2899,38 @@ Qed.
 
 (** CheckLoops function **)
 
-Fixpoint checkloops_comp g p nleft gas {struct gas} :=
+Fixpoint checkloops_comp g p d gas {struct gas} :=
   match gas with
   | O => None
   | S gas' => match p with
               | PEmpty => Some (Some false)
               | PChar _ => Some (Some false)
               | PAnyChar => Some (Some false)
-              | PSequence p1 p2 => match checkloops_comp g p1 nleft gas' with
-                                   | Some (Some false) => checkloops_comp g p2 nleft gas'
+              | PSequence p1 p2 => match checkloops_comp g p1 d gas' with
+                                   | Some (Some false) => checkloops_comp g p2 d gas'
                                    | res => res
                                    end
-              | PChoice p1 p2 => match checkloops_comp g p1 nleft gas' with
-                                 | Some (Some false) => checkloops_comp g p2 nleft gas'
+              | PChoice p1 p2 => match checkloops_comp g p1 d gas' with
+                                 | Some (Some false) => checkloops_comp g p2 d gas'
                                  | res => res
                                  end
-              | PRepetition p' => match nullable_comp g p' nleft gas' with
-                                  | Some (Some false) => checkloops_comp g p' nleft gas'
+              | PRepetition p' => match nullable_comp g p' d gas' with
+                                  | Some (Some false) => checkloops_comp g p' d gas'
                                   | res => res
                                   end
-              | PNot p' => checkloops_comp g p' nleft gas'
+              | PNot p' => checkloops_comp g p' d gas'
               | PNT _ => Some (Some false)
               end
   end.
 
 Lemma checkloops_comp_soundness :
-  forall g p nleft gas res,
-  checkloops_comp g p nleft gas = Some res ->
-  checkloops g p nleft res.
+  forall g p d gas res,
+  checkloops_comp g p d gas = Some res ->
+  checkloops g p d res.
 Proof.
   intros * H.
   generalize dependent res.
-  generalize dependent nleft.
+  generalize dependent d.
   generalize dependent p.
   generalize dependent g.
   induction gas; try discriminate; intros.
@@ -2943,13 +2943,13 @@ Proof.
 Qed.
 
 Lemma checkloops_comp_S_gas :
-  forall g p nleft gas res,
-  checkloops_comp g p nleft gas = Some res ->
-  checkloops_comp g p nleft (S gas) = Some res.
+  forall g p d gas res,
+  checkloops_comp g p d gas = Some res ->
+  checkloops_comp g p d (S gas) = Some res.
 Proof.
   intros * H.
   generalize dependent res.
-  generalize dependent nleft.
+  generalize dependent d.
   generalize dependent p.
   generalize dependent g.
   induction gas; try discriminate; intros.
@@ -2974,10 +2974,10 @@ Proof.
 Qed.
 
 Lemma checkloops_comp_le_gas :
-  forall g p nleft gas gas' res,
-  checkloops_comp g p nleft gas = Some res ->
+  forall g p d gas gas' res,
+  checkloops_comp g p d gas = Some res ->
   gas <= gas' ->
-  checkloops_comp g p nleft gas' = Some res.
+  checkloops_comp g p d gas' = Some res.
 Proof.
   intros * H Hle.
   induction Hle;
@@ -2985,11 +2985,11 @@ Proof.
 Qed.
 
 Lemma checkloops_comp_termination :
-  forall g p nleft,
+  forall g p d,
   (forall r, In r g -> coherent g r true) ->
   coherent g p true ->
   exists gas res,
-  checkloops_comp g p nleft gas = Some res.
+  checkloops_comp g p d gas = Some res.
 Proof.
   intros * Hgc Hpc.
   induction p; intros;
@@ -2998,13 +2998,13 @@ Proof.
   repeat destruct_exists_hyp;
   (* 2 recursive calls *)
   try match goal with
-    [ Hx1: checkloops_comp ?g ?p1 ?nleft ?gas1 = Some ?res1,
-      Hx2: checkloops_comp ?g ?p2 ?nleft ?gas2 = Some ?res2 |- _ ] =>
+    [ Hx1: checkloops_comp ?g ?p1 ?d ?gas1 = Some ?res1,
+      Hx2: checkloops_comp ?g ?p2 ?d ?gas2 = Some ?res2 |- _ ] =>
           assert (gas1 <= gas1 + gas2) by lia;
           assert (gas2 <= gas1 + gas2) by lia;
-          assert (checkloops_comp g p1 nleft (gas1 + gas2) = Some res1)
+          assert (checkloops_comp g p1 d (gas1 + gas2) = Some res1)
           as Hx1' by eauto using checkloops_comp_le_gas;
-          assert (checkloops_comp g p2 nleft (gas1 + gas2) = Some res2)
+          assert (checkloops_comp g p2 d (gas1 + gas2) = Some res2)
           by eauto using checkloops_comp_le_gas;
           exists (1 + gas1 + gas2);
           destruct res1 as [[|]|];
@@ -3015,14 +3015,14 @@ Proof.
   end;
   (* 1 recursive call + nullable_comp *)
   try match goal with
-    [ Hx1: checkloops_comp ?g ?p1 ?nleft ?gas1 = Some ?res1 |- _ ] =>
-        assert (exists gas res, nullable_comp g p1 nleft gas = Some res)
+    [ Hx1: checkloops_comp ?g ?p1 ?d ?gas1 = Some ?res1 |- _ ] =>
+        assert (exists gas res, nullable_comp g p1 d gas = Some res)
         as [gas2 [res2 ?]] by eauto using nullable_comp_termination;
         assert (gas1 <= gas1 + gas2) by lia;
         assert (gas2 <= gas1 + gas2) by lia;
-        assert (checkloops_comp g p1 nleft (gas1 + gas2) = Some res1)
+        assert (checkloops_comp g p1 d (gas1 + gas2) = Some res1)
         as Hx1' by eauto using checkloops_comp_le_gas;
-        assert (nullable_comp g p1 nleft (gas1 + gas2) = Some res2)
+        assert (nullable_comp g p1 d (gas1 + gas2) = Some res2)
         as Hx2' by eauto using nullable_comp_le_gas;
         exists (1 + gas1 + gas2);
         simpl;
@@ -3033,7 +3033,7 @@ Proof.
   end;
   (* 1 recursive call *)
   try match goal with
-    [ Hx1: checkloops_comp ?g ?p1 ?nleft ?gas1 = Some ?res1 |- _ ] =>
+    [ Hx1: checkloops_comp ?g ?p1 ?d ?gas1 = Some ?res1 |- _ ] =>
         exists (1 + gas1);
         simpl;
         eauto;
@@ -3045,17 +3045,17 @@ Qed.
 
 Ltac specialize_checkloops :=
   match goal with
-    [ Hx: checkloops ?g ?p _ ?b, IHx: forall nleft, checkloops ?g ?p nleft ?b -> _ |- _ ] =>
+    [ Hx: checkloops ?g ?p _ ?b, IHx: forall d, checkloops ?g ?p d ?b -> _ |- _ ] =>
         specialize (IHx _ Hx)
   end.
 
 Lemma checkloops_comp_gas_bounded :
-  forall g p gas nleft,
+  forall g p gas d,
   (forall r, In r g -> coherent g r true) ->
   coherent g p true ->
-  gas >= pat_size p + nleft * (grammar_size g) ->
+  gas >= pat_size p + d * (grammar_size g) ->
   exists res,
-  checkloops_comp g p nleft gas = Some res.
+  checkloops_comp g p d gas = Some res.
 Proof.
   intros * Hgc Hpc Hge.
   generalize dependent gas.
@@ -3068,31 +3068,31 @@ Proof.
         inversion Hx
   end;
   try match goal with
-    [ |- exists _, _ ?g (_ ?p) ?nleft (S ?gas) = _ ] =>
-        assert (gas >= pat_size p + nleft * grammar_size g) by lia
+    [ |- exists _, _ ?g (_ ?p) ?d (S ?gas) = _ ] =>
+        assert (gas >= pat_size p + d * grammar_size g) by lia
   end;
   try match goal with
-    [ |- exists _, _ ?g (_ ?p _) ?nleft (S ?gas) = _ ] =>
-        assert (gas >= pat_size p + nleft * grammar_size g) by lia
+    [ |- exists _, _ ?g (_ ?p _) ?d (S ?gas) = _ ] =>
+        assert (gas >= pat_size p + d * grammar_size g) by lia
   end;
   simpl;
   eauto.
   - (* PSequence p1 p2 *)
-    assert (exists res, checkloops_comp g p1 nleft gas = Some res)
+    assert (exists res, checkloops_comp g p1 d gas = Some res)
     as [res1 Hclp1] by eauto.
-    assert (exists res, checkloops_comp g p2 nleft gas = Some res)
+    assert (exists res, checkloops_comp g p2 d gas = Some res)
     as [? ?] by eauto.
     rewrite Hclp1.
     destruct res1 as [[|]|]; eauto.
   - (* PChoice p1 p2 *)
-    assert (exists res, checkloops_comp g p1 nleft gas = Some res)
+    assert (exists res, checkloops_comp g p1 d gas = Some res)
     as [res1 Hclp1] by eauto.
-    assert (exists res, checkloops_comp g p2 nleft gas = Some res)
+    assert (exists res, checkloops_comp g p2 d gas = Some res)
     as [? ?] by eauto.
     rewrite Hclp1.
     destruct res1 as [[|]|]; eauto.
   - (* PRepetition p *)
-    assert (exists res, nullable_comp g p nleft gas = Some res)
+    assert (exists res, nullable_comp g p d gas = Some res)
     as [res Hnp] by eauto using nullable_comp_gas_bounded.
     rewrite Hnp.
     destruct res as [[|]|]; eauto.
@@ -3285,14 +3285,14 @@ Inductive lverifyrule : grammar -> list pat -> bool -> Prop :=
       forall g,
       lverifyrule g nil true
   | LVConsSome :
-      forall g r rs nleft nb v b,
-      verifyrule g r nleft false (Some nb) v ->
+      forall g r rs d nb v b,
+      verifyrule g r d false (Some nb) v ->
       lverifyrule g rs b ->
       lverifyrule g (cons r rs) b
   | LVConsNone :
-      forall g r rs nleft v,
-      length g < nleft ->
-      verifyrule g r nleft false None v ->
+      forall g r rs d v,
+      length g < d ->
+      verifyrule g r d false None v ->
       lverifyrule g (cons r rs) false
   .
 
@@ -3307,17 +3307,17 @@ Proof.
   induction H1; intros;
   inversion H2; subst;
   try match goal with
-    [ HSome : verifyrule ?g ?r ?nleftSome false (Some ?nb') ?vSome,
-      HNone : verifyrule ?g ?r ?nleftNone false None ?vNone,
-      Hlt : length ?g < ?nleftNone |- _ ] =>
-          destruct (Compare_dec.le_ge_dec nleftSome nleftNone);
+    [ HSome : verifyrule ?g ?r ?dSome false (Some ?nb') ?vSome,
+      HNone : verifyrule ?g ?r ?dNone false None ?vNone,
+      Hlt : length ?g < ?dNone |- _ ] =>
+          destruct (Compare_dec.le_ge_dec dSome dNone);
           match goal with
-          | [ Hle : ?nleftSome <= ?nleftNone |- _ ] =>
-                assert (verifyrule g r nleftNone false (Some nb') vSome)
-                by eauto using verifyrule_nleft_le_some_determinism
-          | [ Hle : ?nleftSome >= ?nleftNone |- _ ] =>
-                assert (nleftNone <= nleftSome) by lia;
-                assert (exists v, verifyrule g r nleftSome false None v)
+          | [ Hle : ?dSome <= ?dNone |- _ ] =>
+                assert (verifyrule g r dNone false (Some nb') vSome)
+                by eauto using verifyrule_depth_le_some_determinism
+          | [ Hle : ?dSome >= ?dNone |- _ ] =>
+                assert (dNone <= dSome) by lia;
+                assert (exists v, verifyrule g r dSome false None v)
                 as [? ?] by eauto using verifyrule_convergence
           end;
           pose_verifyrule_determinism;
@@ -3331,8 +3331,8 @@ Lemma lverifyrule_true_In_false :
   forall g rs r,
   lverifyrule g rs true ->
   In r rs ->
-  exists nleft b v,
-  verifyrule g r nleft false (Some b) v.
+  exists d b v,
+  verifyrule g r d false (Some b) v.
 Proof.
   intros * Hlv HIn.
   generalize dependent r.
@@ -3356,14 +3356,14 @@ Lemma lverifyrule_true_In :
   forall g rs r nb,
   lverifyrule g rs true ->
   In r rs ->
-  exists nleft b v,
-  verifyrule g r nleft nb (Some b) v.
+  exists d b v,
+  verifyrule g r d nb (Some b) v.
 Proof.
   intros * Hlv HIn.
-  assert (exists nleft b v, verifyrule g r nleft false (Some b) v)
-  as [nleft [? [v ?]]]
+  assert (exists d b v, verifyrule g r d false (Some b) v)
+  as [d [? [v ?]]]
   by eauto using lverifyrule_true_In_false.
-  assert (exists b', verifyrule g r nleft nb (Some b') v)
+  assert (exists b', verifyrule g r d nb (Some b') v)
   as [? ?]
   by eauto using verifyrule_nb_change_some.
   eauto.
@@ -3402,8 +3402,8 @@ Proof.
           try destruct1;
           try discriminate;
           try match goal with
-            [ Hx: verifyrule_comp ?g ?r ?nleft false ?gas = Some (?res, ?v) |- _ ] =>
-                assert (verifyrule g r nleft false res v)
+            [ Hx: verifyrule_comp ?g ?r ?d false ?gas = Some (?res, ?v) |- _ ] =>
+                assert (verifyrule g r d false res v)
                 by eauto using verifyrule_comp_soundness
           end;
           eauto using lverifyrule
@@ -3428,8 +3428,8 @@ Proof.
           try discriminate;
           try destruct1;
           match goal with
-            [ Hx: verifyrule_comp ?g ?r ?nleft ?nb ?gas = Some ?res |- _ ] =>
-                assert (verifyrule_comp g r nleft nb (S gas) = Some res)
+            [ Hx: verifyrule_comp ?g ?r ?d ?nb ?gas = Some ?res |- _ ] =>
+                assert (verifyrule_comp g r d nb (S gas) = Some res)
                 as ? by eauto using verifyrule_comp_S_gas;
                 unfold lverifyrule_comp;
                 rewrite_match_subject_in_goal;
@@ -3534,12 +3534,12 @@ Inductive lcheckloops : grammar -> list pat -> bool -> Prop :=
       forall g,
       lcheckloops g nil false
   | LCLConsSomeTrue :
-      forall g r nleft rs,
-      checkloops g r nleft (Some true) ->
+      forall g r d rs,
+      checkloops g r d (Some true) ->
       lcheckloops g (cons r rs) true
   | LCLConsSomeFalse :
-      forall g r nleft rs b,
-      checkloops g r nleft (Some false) ->
+      forall g r d rs b,
+      checkloops g r d (Some false) ->
       lcheckloops g rs b ->
       lcheckloops g (cons r rs) b
   .
@@ -3555,8 +3555,8 @@ Proof.
   induction H1; intros;
   inversion H2; subst;
   try match goal with
-    [ Hx1: checkloops ?g ?r ?nleft1 (Some ?b1),
-      Hx2: checkloops ?g ?r ?nleft2 (Some ?b2) |- _ ] =>
+    [ Hx1: checkloops ?g ?r ?d1 (Some ?b1),
+      Hx2: checkloops ?g ?r ?d2 (Some ?b2) |- _ ] =>
           assert (b1 = b2)
           by eauto using checkloops_Some_determinism
   end;
@@ -3568,8 +3568,8 @@ Lemma lcheckloops_false_In :
   forall g rs r,
   lcheckloops g rs false ->
   In r rs ->
-  exists nleft,
-  checkloops g r nleft (Some false).
+  exists d,
+  checkloops g r d (Some false).
 Proof.
   intros * Hcl HIn.
   generalize dependent r.
@@ -3619,8 +3619,8 @@ Proof.
           try destruct1;
           try discriminate;
           try match goal with
-            [ Hx: checkloops_comp ?g ?r ?nleft ?gas = Some ?res |- _ ] =>
-                assert (checkloops g r nleft res)
+            [ Hx: checkloops_comp ?g ?r ?d ?gas = Some ?res |- _ ] =>
+                assert (checkloops g r d res)
                 by eauto using checkloops_comp_soundness
           end;
           eauto using lcheckloops
@@ -3649,8 +3649,8 @@ Proof.
           try discriminate;
           try destruct1;
           try match goal with
-            [ Hx: checkloops_comp ?g ?r ?nleft ?gas = Some ?res |- _ ] =>
-                assert (checkloops_comp g r nleft (S gas) = Some res)
+            [ Hx: checkloops_comp ?g ?r ?d ?gas = Some ?res |- _ ] =>
+                assert (checkloops_comp g r d (S gas) = Some res)
                 as ? by eauto using checkloops_comp_S_gas;
                 unfold lcheckloops_comp;
                 rewrite_match_subject_in_goal;
@@ -3692,8 +3692,8 @@ Proof.
       [ Hx: lcoherent ?g ?rs true -> _, Hy: lcoherent ?g ?rs true |- _ ] =>
           specialize (Hx Hy) as [gas1 [resrs ?]]
     end.
-    assert (exists nleft b, checkloops g r nleft (Some b))
-    as [nleft [b ?]]
+    assert (exists d b, checkloops g r d (Some b))
+    as [d [b ?]]
     by eauto using checkloops_safe_grammar, lcoherent_true_In, lverifyrule_true_In.
     assert (exists gas res, checkloops_comp g r (S (length g)) gas = Some res)
     as [gas2 [res Hcl]]
@@ -3738,8 +3738,8 @@ Proof.
   assert (exists b, checkloops_comp g r (S (length g)) gas = Some b)
   as [clres Hcl] by eauto using checkloops_comp_gas_bounded, lcoherent_true_In.
   rewrite Hcl.
-  assert (exists nleft b, checkloops g r nleft (Some b))
-  as [nleft [b ?]]
+  assert (exists d b, checkloops g r d (Some b))
+  as [d [b ?]]
   by eauto using checkloops_safe_grammar, lcoherent_true_In, lverifyrule_true_In.
   assert (checkloops g r (S (length g)) clres)
   by eauto using checkloops_comp_soundness.
@@ -3997,16 +3997,16 @@ Inductive verifygrammarpat : grammar -> pat -> bool -> Prop :=
       coherent g p false ->
       verifygrammarpat g p false
   | VGPPatWithEmptyLoop :
-      forall g p nleft,
+      forall g p d,
       verifygrammar g true ->
       coherent g p true ->
-      checkloops g p nleft (Some true) ->
+      checkloops g p d (Some true) ->
       verifygrammarpat g p false
   | VGPSafe :
-      forall g p nleft,
+      forall g p d,
       verifygrammar g true ->
       coherent g p true ->
-      checkloops g p nleft (Some false) ->
+      checkloops g p d (Some false) ->
       verifygrammarpat g p true
   .
 
@@ -4030,7 +4030,7 @@ Qed.
 Lemma verifygrammarpat_true :
   forall g p,
   verifygrammarpat g p true ->
-  verifygrammar g true /\ coherent g p true /\ exists nleft, checkloops g p nleft (Some false).
+  verifygrammar g true /\ coherent g p true /\ exists d, checkloops g p d (Some false).
 Proof.
   intros * H.
   inversion H;
@@ -4095,9 +4095,9 @@ Proof.
         )
   end;
   try match goal with
-    [ Hx: checkloops_comp ?g ?p ?nleft ?gas = Some ?b |- _ ] =>
+    [ Hx: checkloops_comp ?g ?p ?d ?gas = Some ?b |- _ ] =>
         let H := fresh in (
-          assert (checkloops_comp g p nleft (S gas) = Some b)
+          assert (checkloops_comp g p d (S gas) = Some b)
           as H
           by eauto using checkloops_comp_S_gas;
           rewrite H;
@@ -4140,14 +4140,14 @@ Proof.
     by eauto using coherent_comp_soundness.
     destruct bc.
     + (* true *)
-      pose (S (length g)) as nleft.
-      assert (exists gas b, checkloops_comp g p nleft gas = Some b)
+      pose (S (length g)) as d.
+      assert (exists gas b, checkloops_comp g p d gas = Some b)
       as [gasl [rescl ?]]
       by eauto using checkloops_comp_termination, lcoherent_true_In.
-      assert (checkloops g p nleft rescl)
+      assert (checkloops g p d rescl)
       by eauto using checkloops_comp_soundness.
-      assert (exists nleft b, checkloops g p nleft (Some b))
-      as [nleft' [bl' ?]]
+      assert (exists d b, checkloops g p d (Some b))
+      as [d' [bl' ?]]
       by eauto using checkloops_safe_grammar, lcoherent_true_In, lverifyrule_true_In.
       assert (rescl = Some bl')
       by eauto using checkloops_Some_convergence, lcoherent_true_In, lverifyrule_true_In.
@@ -4165,10 +4165,10 @@ Proof.
       as Hc'
       by eauto using coherent_comp_le_gas.
       rewrite Hc'.
-      assert (checkloops_comp g p nleft gas = Some (Some bl'))
+      assert (checkloops_comp g p d gas = Some (Some bl'))
       as Hl'
       by eauto using checkloops_comp_le_gas.
-      subst nleft.
+      subst d.
       rewrite Hl'.
       destruct bl';
       eauto.
@@ -4221,8 +4221,8 @@ Proof.
   assert (gas >= pat_size p + S (length g) * grammar_size g) by lia.
   assert (exists b, checkloops_comp g p (S (length g)) gas = Some b)
   as [rescl Hcl] by eauto using checkloops_comp_gas_bounded, lcoherent_true_In.
-  assert (exists nleft b, checkloops g p nleft (Some b))
-  as [nleft [b ?]]
+  assert (exists d b, checkloops g p d (Some b))
+  as [d [b ?]]
   by eauto using checkloops_safe_grammar, lcoherent_true_In, lverifyrule_true_In.
   assert (checkloops g p (S (length g)) rescl)
   by eauto using checkloops_comp_soundness.
@@ -4260,29 +4260,29 @@ Proof.
 Qed.
 
 Theorem safe_match :
-  forall g p nleft s,
+  forall g p d s,
   (forall r, In r g -> coherent g r true) ->
-  (forall r nb, In r g -> exists nleft b v, verifyrule g r nleft nb (Some b) v) ->
-  (forall r, In r g -> exists nleft, checkloops g r nleft (Some false)) ->
+  (forall r nb, In r g -> exists d b v, verifyrule g r d nb (Some b) v) ->
+  (forall r, In r g -> exists d, checkloops g r d (Some false)) ->
   coherent g p true ->
-  checkloops g p nleft (Some false) ->
+  checkloops g p d (Some false) ->
   exists res, matches g p s res.
 Proof.
   intros * Hcg Hvg Hclg Hcp Hclp.
   remember (String.length s) as n.
   generalize dependent s.
-  generalize dependent nleft.
+  generalize dependent d.
   generalize dependent p.
   generalize dependent g.
   induction n using strong_induction;
   intros.
-  assert (exists nb nleft' b v, verifyrule g p nleft' nb (Some b) v)
+  assert (exists nb d' b v, verifyrule g p d' nb (Some b) v)
   as [nb [? [b [? Hvp]]]]
   by (exists true; eauto using verifyrule_safe_grammar_yields_safe_pattern).
   remember (Some b) as res in Hvp.
   generalize dependent b.
   generalize dependent s.
-  generalize dependent nleft.
+  generalize dependent d.
   generalize dependent n.
   induction Hvp;
   intros;
@@ -4325,8 +4325,8 @@ Proof.
     eauto using matches.
   - (* PSequence p1 p2, with non-nullable p1 *)
     match goal with
-      [ _: verifyrule ?g p1 ?nleft false (Some false) _ |- _ ] =>
-          assert (nullable g p1 nleft (Some false))
+      [ _: verifyrule ?g p1 ?d false (Some false) _ |- _ ] =>
+          assert (nullable g p1 d (Some false))
           by eauto using verifyrule_similar_to_nullable
     end.
     assert (exists res, matches g p1 s res) as [res1 ?] by eauto.
@@ -4360,29 +4360,29 @@ Proof.
     eauto using matches.
   - (* PNT i *)
     assert (In p g) by eauto using nth_error_In.
-    assert (exists nleft, checkloops g p nleft (Some false))
+    assert (exists d, checkloops g p d (Some false))
     as [? ?] by eauto.
     assert (exists res, matches g p s res) as [? ?] by eauto.
     eauto using matches.
 Qed.
 
 Theorem lpredicates_safe_match :
-  forall g p nleft s,
+  forall g p d s,
   lcoherent g g true ->
   lverifyrule g g true ->
   lcheckloops g g false ->
   coherent g p true ->
-  checkloops g p nleft (Some false) ->
+  checkloops g p d (Some false) ->
   exists res, matches g p s res.
 Proof.
   eauto using safe_match, lcoherent_true_In, lverifyrule_true_In, lcheckloops_false_In.
 Qed.
 
 Theorem verifygrammar_safe_match :
-  forall g p nleft s,
+  forall g p d s,
   verifygrammar g true ->
   coherent g p true ->
-  checkloops g p nleft (Some false) ->
+  checkloops g p d (Some false) ->
   exists res, matches g p s res.
 Proof.
   intros * Hvg Hpc Hlp.
